template-coq/theories/Typing.v
@@ -591,68 +591,73 @@ Module TemplateConversionPar <: ConversionParSig TemplateTerm Env TemplateTermUt
   Definition cumul_gen := @cumul_gen.
 End TemplateConversionPar.
 
-
+(* TODO : add rules for named contexts. *)
 Class GuardChecker :=
 { (* Structural recursion check *)
-  fix_guard : global_env_ext -> context -> mfixpoint term -> bool ;
+  fix_guard : global_env_ext -> named_context -> context -> mfixpoint term -> bool ;
   (* Guarded by destructors check *)
-  cofix_guard : global_env_ext -> context -> mfixpoint term -> bool ;
+  cofix_guard : global_env_ext -> named_context -> context -> mfixpoint term -> bool ;
 
-  fix_guard_red1 Σ Γ mfix mfix' idx :
-      fix_guard Σ Γ mfix ->
-      red1 Σ Γ (tFix mfix idx) (tFix mfix' idx) ->
-      fix_guard Σ Γ mfix' ;
+  fix_guard_red1 Σ Δ Γ mfix mfix' idx :
+      fix_guard Σ Δ Γ mfix ->
+      red1 Σ Δ Γ (tFix mfix idx) (tFix mfix' idx) ->
+      fix_guard Σ Δ Γ mfix' ;
 
-  fix_guard_lift Σ Γ Γ' Γ'' mfix :
+  fix_guard_lift Σ Δ Γ Γ' Γ'' mfix :
     let k' := (#|mfix| + #|Γ'|)%nat in
     let mfix' := map (map_def (lift #|Γ''| #|Γ'|) (lift #|Γ''| k')) mfix in
-    fix_guard Σ (Γ ,,, Γ') mfix ->
-    fix_guard Σ (Γ ,,, Γ'' ,,, lift_context #|Γ''| 0 Γ') mfix' ;
+    fix_guard Σ Δ (Γ ,,, Γ') mfix ->
+    fix_guard Σ Δ (Γ ,,, Γ'' ,,, lift_context #|Γ''| 0 Γ') mfix' ;
 
-  fix_guard_subst Σ Γ Γ' Δ mfix s k :
+  (*
+  fix_guard_lift' Σ Δ Δ' Δ'' Γ mfix :
+    fix_guard Σ (Δ ,,, Δ') Γ mfix ->
+    fix_guard Σ (Δ ,,, Δ'' ,,, Δ') Γ mfix ;*)
+
+  fix_guard_subst Σ Δ Γ Γ' Γ0 mfix s k :
     let k' := (#|mfix| + k)%nat in
     let mfix' := map (map_def (subst s k) (subst s k')) mfix in
-    fix_guard Σ (Γ ,,, Γ' ,,, Δ) mfix ->
-    fix_guard Σ (Γ ,,, subst_context s 0 Δ) mfix' ;
+    fix_guard Σ Δ (Γ ,,, Γ' ,,, Γ0) mfix ->
+    fix_guard Σ Δ (Γ ,,, subst_context s 0 Γ0) mfix' ;
 
-  fix_guard_subst_instance {cf:checker_flags} Σ Γ mfix u univs :
+  fix_guard_subst_instance {cf:checker_flags} Σ Δ Γ mfix u univs :
     consistent_instance_ext (Σ.1, univs) Σ.2 u ->
-    fix_guard Σ Γ mfix ->
-    fix_guard (Σ.1, univs) (subst_instance u Γ) (map (map_def (subst_instance u) (subst_instance u))
+    fix_guard Σ Δ Γ mfix ->
+    fix_guard (Σ.1, univs) Δ (subst_instance u Γ) (map (map_def (subst_instance u) (subst_instance u))
                     mfix) ;
 
-  fix_guard_extends Σ Γ mfix (Σ' : global_env_ext) :
-    fix_guard Σ Γ mfix ->
+  fix_guard_extends Σ Δ Γ mfix (Σ' : global_env_ext) :
+    fix_guard Σ Δ Γ mfix ->
     extends Σ.1 Σ' ->
-    fix_guard Σ' Γ mfix ;
+    fix_guard Σ' Δ Γ mfix ;
 
-  cofix_guard_red1 Σ Γ mfix mfix' idx :
-    cofix_guard Σ Γ mfix ->
-    red1 Σ Γ (tCoFix mfix idx) (tCoFix mfix' idx) ->
-    cofix_guard Σ Γ mfix' ;
+  cofix_guard_red1 Σ Δ Γ mfix mfix' idx :
+    cofix_guard Σ Δ Γ mfix ->
+    red1 Σ Δ Γ (tCoFix mfix idx) (tCoFix mfix' idx) ->
+    cofix_guard Σ Δ Γ mfix' ;
 
-  cofix_guard_lift Σ Γ Γ' Γ'' mfix :
+  cofix_guard_lift Σ Δ Γ Γ' Γ'' mfix :
     let k' := (#|mfix| + #|Γ'|)%nat in
     let mfix' := map (map_def (lift #|Γ''| #|Γ'|) (lift #|Γ''| k')) mfix in
-    cofix_guard Σ (Γ ,,, Γ') mfix ->
-    cofix_guard Σ (Γ ,,, Γ'' ,,, lift_context #|Γ''| 0 Γ') mfix' ;
+    cofix_guard Σ Δ (Γ ,,, Γ') mfix ->
+    cofix_guard Σ Δ (Γ ,,, Γ'' ,,, lift_context #|Γ''| 0 Γ') mfix' ;
 
-  cofix_guard_subst Σ Γ Γ' Δ mfix s k :
+  cofix_guard_subst Σ Δ Γ Γ' Γ0 mfix s k :
     let k' := (#|mfix| + k)%nat in
     let mfix' := map (map_def (subst s k) (subst s k')) mfix in
-    cofix_guard Σ (Γ ,,, Γ' ,,, Δ) mfix ->
-    cofix_guard Σ (Γ ,,, subst_context s 0 Δ) mfix' ;
+    cofix_guard Σ Δ (Γ ,,, Γ' ,,, Γ0) mfix ->
+    cofix_guard Σ Δ (Γ ,,, subst_context s 0 Γ0) mfix' ;
 
-  cofix_guard_subst_instance {cf:checker_flags} Σ Γ mfix u univs :
+  cofix_guard_subst_instance {cf:checker_flags} Σ Δ Γ mfix u univs :
     consistent_instance_ext (Σ.1, univs) Σ.2 u ->
-    cofix_guard Σ Γ mfix ->
-    cofix_guard (Σ.1, univs) (subst_instance u Γ) (map (map_def (subst_instance u) (subst_instance u))
+    cofix_guard Σ Δ Γ mfix ->
+    cofix_guard (Σ.1, univs) Δ (subst_instance u Γ) (map (map_def (subst_instance u) (subst_instance u))
                     mfix) ;
 
-  cofix_guard_extends Σ Γ mfix (Σ' : global_env_ext) :
-    cofix_guard Σ Γ mfix ->
+  cofix_guard_extends Σ Δ Γ mfix (Σ' : global_env_ext) :
+    cofix_guard Σ Δ Γ mfix ->
     extends Σ.1 Σ' ->
-    cofix_guard Σ' Γ mfix }.
+    cofix_guard Σ' Δ Γ mfix }.
 
 (* AXIOM GUARD CONDITION *)
 Axiom guard_checking : GuardChecker.
@@ -783,62 +788,68 @@ Definition wf_cofixpoint (Σ : global_env) mfix :=
   | _ => false
   end.
 
-Reserved Notation "'wf_local' Σ Γ " (at level 9, Σ, Γ at next level).
+Reserved Notation "'wf_named' Σ Δ " (at level 9, Σ, Δ at next level).
+Reserved Notation "'wf_local' Σ Δ Γ " (at level 9, Σ, Δ, Γ at next level).
 
-Inductive typing `{checker_flags} (Σ : global_env_ext) (Γ : context) : term -> term -> Type :=
+Inductive typing `{checker_flags} (Σ : global_env_ext) (Δ : named_context) (Γ : context) : term -> term -> Type :=
 | type_Rel n decl :
-    wf_local Σ Γ ->
+    wf_named Σ Δ -> wf_local Σ Δ Γ ->
     nth_error Γ n = Some decl ->
-    Σ ;;; Γ |- tRel n : lift0 (S n) decl.(decl_type)
+    Σ ;;; Δ ;;; Γ |- tRel n : lift0 (S n) decl.(decl_type)
+
+| type_Var id decl : 
+    wf_named Σ Δ -> wf_local Σ Δ Γ ->
+    nctx_lookup Δ id = Some decl ->
+    Σ ;;; Δ ;;; Γ |- tVar id : decl.(decl_type)
 
 | type_Sort s :
-    wf_local Σ Γ ->
+    wf_named Σ Δ -> wf_local Σ Δ Γ ->
     wf_sort Σ s ->
-    Σ ;;; Γ |- tSort s : tSort (Sort.super s)
+    Σ ;;; Δ ;;; Γ |- tSort s : tSort (Sort.super s)
 
 | type_Cast c k t s :
-    Σ ;;; Γ |- t : tSort s ->
-    Σ ;;; Γ |- c : t ->
-    Σ ;;; Γ |- tCast c k t : t
+    Σ ;;; Δ ;;; Γ |- t : tSort s ->
+    Σ ;;; Δ ;;; Γ |- c : t ->
+    Σ ;;; Δ ;;; Γ |- tCast c k t : t
 
 | type_Prod na t b s1 s2 :
-    lift_typing typing Σ Γ (j_vass_s na t s1) ->
-    Σ ;;; Γ ,, vass na t |- b : tSort s2 ->
-    Σ ;;; Γ |- tProd na t b : tSort (Sort.sort_of_product s1 s2)
+    lift_typing3 typing Σ Δ Γ (j_vass_s na t s1) ->
+    Σ ;;; Δ ;;; Γ ,, vass na t |- b : tSort s2 ->
+    Σ ;;; Δ ;;; Γ |- tProd na t b : tSort (Sort.sort_of_product s1 s2)
 
 | type_Lambda na t b bty :
-    lift_typing typing Σ Γ (j_vass na t) ->
-    Σ ;;; Γ ,, vass na t |- b : bty ->
-    Σ ;;; Γ |- tLambda na t b : tProd na t bty
+    lift_typing3 typing Σ Δ Γ (j_vass na t) ->
+    Σ ;;; Δ ;;; Γ ,, vass na t |- b : bty ->
+    Σ ;;; Δ ;;; Γ |- tLambda na t b : tProd na t bty
 
 | type_LetIn na b b_ty b' b'_ty :
-    lift_typing typing Σ Γ (j_vdef na b b_ty) ->
-    Σ ;;; Γ ,, vdef na b b_ty |- b' : b'_ty ->
-    Σ ;;; Γ |- tLetIn na b b_ty b' : tLetIn na b b_ty b'_ty
+    lift_typing3 typing Σ Δ Γ (j_vdef na b b_ty) ->
+    Σ ;;; Δ ;;; Γ ,, vdef na b b_ty |- b' : b'_ty ->
+    Σ ;;; Δ ;;; Γ |- tLetIn na b b_ty b' : tLetIn na b b_ty b'_ty
 
 | type_App t l t_ty t' :
-    Σ ;;; Γ |- t : t_ty ->
+    Σ ;;; Δ ;;; Γ |- t : t_ty ->
     isApp t = false -> l <> [] -> (* Well-formed application *)
-    typing_spine Σ Γ t_ty l t' ->
-    Σ ;;; Γ |- tApp t l : t'
+    typing_spine Σ Δ Γ t_ty l t' ->
+    Σ ;;; Δ ;;; Γ |- tApp t l : t'
 
 | type_Const cst u :
-    wf_local Σ Γ ->
+    wf_named Σ Δ -> wf_local Σ Δ Γ ->
     forall decl (isdecl : declared_constant Σ.1 cst decl),
     consistent_instance_ext Σ decl.(cst_universes) u ->
-    Σ ;;; Γ |- (tConst cst u) : subst_instance u decl.(cst_type)
+    Σ ;;; Δ ;;; Γ |- (tConst cst u) : subst_instance u decl.(cst_type)
 
 | type_Ind ind u :
-    wf_local Σ Γ ->
+    wf_named Σ Δ -> wf_local Σ Δ Γ ->
     forall mdecl idecl (isdecl : declared_inductive Σ.1 ind mdecl idecl),
     consistent_instance_ext Σ mdecl.(ind_universes) u ->
-    Σ ;;; Γ |- (tInd ind u) : subst_instance u idecl.(ind_type)
+    Σ ;;; Δ ;;; Γ |- (tInd ind u) : subst_instance u idecl.(ind_type)
 
 | type_Construct ind i u :
-    wf_local Σ Γ ->
+    wf_named Σ Δ -> wf_local Σ Δ Γ ->
     forall mdecl idecl cdecl (isdecl : declared_constructor Σ.1 (ind, i) mdecl idecl cdecl),
     consistent_instance_ext Σ mdecl.(ind_universes) u ->
-    Σ ;;; Γ |- (tConstruct ind i u) : type_of_constructor mdecl cdecl (ind, i) u
+    Σ ;;; Δ ;;; Γ |- (tConstruct ind i u) : type_of_constructor mdecl cdecl (ind, i) u
 
 | type_Case (ci : case_info) p c brs indices ps :
     forall mdecl idecl (isdecl : declared_inductive Σ.1 ci.(ci_ind) mdecl idecl),
@@ -847,95 +858,97 @@ Inductive typing `{checker_flags} (Σ : global_env_ext) (Γ : context) : term ->
     context_assumptions mdecl.(ind_params) = #|p.(pparams)| ->
     consistent_instance_ext Σ (ind_universes mdecl) p.(puinst) ->
     let predctx := case_predicate_context ci.(ci_ind) mdecl idecl p in
-    ctx_inst (typing Σ) Γ (p.(pparams) ++ indices)
+    ctx_inst (typing Σ Δ) Γ (p.(pparams) ++ indices)
       (List.rev (ind_params mdecl ,,, ind_indices idecl : context)@[p.(puinst)]) ->
-    Σ ;;; Γ ,,, predctx |- p.(preturn) : tSort ps ->
+    Σ ;;; Δ ;;; Γ ,,, predctx |- p.(preturn) : tSort ps ->
     is_allowed_elimination Σ idecl.(ind_kelim) ps ->
-    Σ ;;; Γ |- c : mkApps (tInd ci.(ci_ind) p.(puinst)) (p.(pparams) ++ indices) ->
+    Σ ;;; Δ ;;; Γ |- c : mkApps (tInd ci.(ci_ind) p.(puinst)) (p.(pparams) ++ indices) ->
     isCoFinite mdecl.(ind_finite) = false ->
     let ptm := it_mkLambda_or_LetIn predctx p.(preturn) in
     All2i (fun i cdecl br =>
       let brctxty := case_branch_type ci.(ci_ind) mdecl p ptm i cdecl br in
       (wf_nactx br.(bcontext) (cstr_branch_context ci.(ci_ind) mdecl cdecl)) *
-      (Σ ;;; Γ ,,, brctxty.1 |- br.(bbody) : brctxty.2) *
-      (Σ ;;; Γ ,,, brctxty.1 |- brctxty.2 : tSort ps))
+      (Σ ;;; Δ ;;; Γ ,,, brctxty.1 |- br.(bbody) : brctxty.2) *
+      (Σ ;;; Δ ;;; Γ ,,, brctxty.1 |- brctxty.2 : tSort ps))
       0 idecl.(ind_ctors) brs ->
-    Σ ;;; Γ |- tCase ci p c brs : mkApps ptm (indices ++ [c])
+    Σ ;;; Δ ;;; Γ |- tCase ci p c brs : mkApps ptm (indices ++ [c])
 
 | type_Proj p c u :
     forall mdecl idecl cdecl pdecl (isdecl : declared_projection Σ.1 p mdecl idecl cdecl pdecl) args,
-    Σ ;;; Γ |- c : mkApps (tInd p.(proj_ind) u) args ->
+    Σ ;;; Δ ;;; Γ |- c : mkApps (tInd p.(proj_ind) u) args ->
     #|args| = ind_npars mdecl ->
-    Σ ;;; Γ |- tProj p c : subst0 (c :: List.rev args) (subst_instance u pdecl.(proj_type))
+    Σ ;;; Δ ;;; Γ |- tProj p c : subst0 (c :: List.rev args) (subst_instance u pdecl.(proj_type))
 
 | type_Fix mfix n decl :
-    fix_guard Σ Γ mfix ->
+    fix_guard Σ Δ Γ mfix ->
     nth_error mfix n = Some decl ->
-    wf_local Σ Γ ->
-    All (on_def_type (lift_typing1 (typing Σ)) Γ) mfix ->
-    All (on_def_body (lift_typing1 (typing Σ)) (fix_context mfix) Γ) mfix ->
+    wf_named Σ Δ -> wf_local Σ Δ Γ ->
+    All (on_def_type (lift_typing1 (typing Σ Δ)) Γ) mfix ->
+    All (on_def_body (lift_typing1 (typing Σ Δ)) (fix_context mfix) Γ) mfix ->
     wf_fixpoint Σ mfix ->
-      Σ ;;; Γ |- tFix mfix n : decl.(dtype)
+      Σ ;;; Δ ;;; Γ |- tFix mfix n : decl.(dtype)
 
 | type_CoFix mfix n decl :
-    cofix_guard Σ Γ mfix ->
+    cofix_guard Σ Δ Γ mfix ->
     nth_error mfix n = Some decl ->
-    wf_local Σ Γ ->
-    All (on_def_type (lift_typing1 (typing Σ)) Γ) mfix ->
-    All (on_def_body (lift_typing1 (typing Σ)) (fix_context mfix) Γ) mfix ->
+    wf_named Σ Δ -> wf_local Σ Δ Γ ->
+    All (on_def_type (lift_typing1 (typing Σ Δ)) Γ) mfix ->
+    All (on_def_body (lift_typing1 (typing Σ Δ)) (fix_context mfix) Γ) mfix ->
     wf_cofixpoint Σ mfix ->
-    Σ ;;; Γ |- tCoFix mfix n : decl.(dtype)
+    Σ ;;; Δ ;;; Γ |- tCoFix mfix n : decl.(dtype)
 
 | type_Int p prim_ty cdecl :
-    wf_local Σ Γ ->
+    wf_named Σ Δ -> wf_local Σ Δ Γ ->
     primitive_constant Σ primInt = Some prim_ty ->
     declared_constant Σ prim_ty cdecl ->
     primitive_invariants primInt cdecl ->
-    Σ ;;; Γ |- tInt p : tConst prim_ty []
+    Σ ;;; Δ ;;; Γ |- tInt p : tConst prim_ty []
 
 | type_Float p prim_ty cdecl :
-    wf_local Σ Γ ->
+    wf_named Σ Δ -> wf_local Σ Δ Γ ->
     primitive_constant Σ primFloat = Some prim_ty ->
     declared_constant Σ prim_ty cdecl ->
     primitive_invariants primFloat cdecl ->
-    Σ ;;; Γ |- tFloat p : tConst prim_ty []
+    Σ ;;; Δ ;;; Γ |- tFloat p : tConst prim_ty []
 
 | type_String p prim_ty cdecl :
-    wf_local Σ Γ ->
+    wf_named Σ Δ -> wf_local Σ Δ Γ ->
     primitive_constant Σ primString = Some prim_ty ->
     declared_constant Σ prim_ty cdecl ->
     primitive_invariants primString cdecl ->
-    Σ ;;; Γ |- tString p : tConst prim_ty []
+    Σ ;;; Δ ;;; Γ |- tString p : tConst prim_ty []
 
 | type_Array prim_ty cdecl u arr def ty :
-    wf_local Σ Γ ->
+    wf_named Σ Δ -> wf_local Σ Δ Γ ->
     primitive_constant Σ primArray = Some prim_ty ->
     declared_constant Σ prim_ty cdecl ->
     primitive_invariants primArray cdecl ->
     let s := sType (Universe.make' u) in
-    Σ ;;; Γ |- ty : tSort s ->
-    Σ ;;; Γ |- def : ty ->
-    All (fun t => Σ ;;; Γ |- t : ty) arr ->
-    Σ ;;; Γ |- tArray u arr def ty : tApp (tConst prim_ty [u]) [ty]
+    Σ ;;; Δ ;;; Γ |- ty : tSort s ->
+    Σ ;;; Δ ;;; Γ |- def : ty ->
+    All (fun t => Σ ;;; Δ ;;; Γ |- t : ty) arr ->
+    Σ ;;; Δ ;;; Γ |- tArray u arr def ty : tApp (tConst prim_ty [u]) [ty]
 
 | type_Conv t A B s :
-    Σ ;;; Γ |- t : A ->
-    Σ ;;; Γ |- B : tSort s ->
-    Σ ;;; Γ |- A <= B -> Σ ;;; Γ |- t : B
+    Σ ;;; Δ ;;; Γ |- t : A ->
+    Σ ;;; Δ ;;; Γ |- B : tSort s ->
+    Σ ;;; Δ ;;; Γ |- A <= B -> 
+    Σ ;;; Δ ;;; Γ |- t : B
 
-where " Σ ;;; Γ |- t : T " := (typing Σ Γ t T) : type_scope
-  and "'wf_local' Σ Γ " := (All_local_env (lift_typing1 (typing Σ)) Γ) : type_scope
+where " Σ ;;; Δ ;;; Γ |- t : T " := (typing Σ Δ Γ t T) : type_scope
+  and "'wf_named' Σ Δ " := (All_named_env (lift_typing2 (typing Σ)) Δ) : type_scope
+  and "'wf_local' Σ Δ Γ " := (All_local_env (lift_typing1 (typing Σ Δ)) Γ) : type_scope
 
 (* Typing of "spines", currently just the arguments of applications *)
 
-with typing_spine `{checker_flags} (Σ : global_env_ext) (Γ : context) : term -> list term -> term -> Type :=
-| type_spine_nil ty : typing_spine Σ Γ ty [] ty
+with typing_spine `{checker_flags} (Σ : global_env_ext) (Δ : named_context) (Γ : context) : term -> list term -> term -> Type :=
+| type_spine_nil ty : typing_spine Σ Δ Γ ty [] ty
 | type_spine_cons hd tl na A B s T B' :
-    Σ ;;; Γ |- tProd na A B : tSort s ->
-    Σ ;;; Γ |- T <= tProd na A B ->
-    Σ ;;; Γ |- hd : A ->
-    typing_spine Σ Γ (subst10 hd B) tl B' ->
-    typing_spine Σ Γ T (cons hd tl) B'.
+    Σ ;;; Δ ;;; Γ |- tProd na A B : tSort s ->
+    Σ ;;; Δ ;;; Γ |- T <= tProd na A B ->
+    Σ ;;; Δ ;;; Γ |- hd : A ->
+    typing_spine Σ Δ Γ (subst10 hd B) tl B' ->
+    typing_spine Σ Δ Γ T (cons hd tl) B'.
 
 Derive Signature for typing typing_spine.
 
@@ -971,77 +984,70 @@ Include TemplateDeclarationTyping.
 
 Section Typing_Spine_size.
   Context `{checker_flags}.
-  Context (fn : forall (Σ : global_env_ext) (Γ : context) (t T : term), typing Σ Γ t T -> size).
-  Context (Σ : global_env_ext) (Γ : context).
+  Context (fn : forall (Σ : global_env_ext) (Δ : named_context) (Γ : context) (t T : term), typing Σ Δ Γ t T -> size).
+  Context (Σ : global_env_ext) (Δ : named_context) (Γ : context).
 
-  Fixpoint typing_spine_size t T U (s : typing_spine Σ Γ t T U) : size :=
+  Fixpoint typing_spine_size t T U (s : typing_spine Σ Δ Γ t T U) : size :=
   match s with
   | type_spine_nil _ => 0
   | type_spine_cons hd tl na A B s T B' typrod cumul ty s' =>
-    (fn _ _ _ _ ty + fn _ _ _ _ typrod + typing_spine_size _ _ _ s')%nat
+    (fn _ _ _ _ _ ty + fn _ _ _ _ _ typrod + typing_spine_size _ _ _ s')%nat
   end.
 End Typing_Spine_size.
 
 Section CtxInstSize.
-  Context (typing : global_env_ext -> context -> term -> term -> Type)
-  (typing_size : forall {Σ Γ t T}, typing Σ Γ t T -> size).
+  Context (typing : global_env_ext -> named_context -> context -> term -> term -> Type)
+  (typing_size : forall {Σ Δ Γ t T}, typing Σ Δ Γ t T -> size).
 
-  Fixpoint ctx_inst_size {Σ Γ args Δ} (c : ctx_inst (typing Σ) Γ args Δ) : size :=
+  Fixpoint ctx_inst_size {Σ Δ Γ args Γ0} (c : ctx_inst (typing Σ Δ) Γ args Γ0) : size :=
   match c with
   | ctx_inst_nil => 0
-  | ctx_inst_ass na t i inst Δ ty ctxi => ((typing_size _ _ _ _ ty) + (ctx_inst_size ctxi))%nat
-  | ctx_inst_def na b t inst Δ ctxi => S (ctx_inst_size ctxi)
+  | ctx_inst_ass na t i inst Γ0 ty ctxi => ((typing_size _ _ _ _ _ ty) + (ctx_inst_size ctxi))%nat
+  | ctx_inst_def na b t inst Γ0 ctxi => S (ctx_inst_size ctxi)
   end.
 
 End CtxInstSize.
 
-Definition typing_size `{checker_flags} {Σ Γ t T} (d : Σ ;;; Γ |- t : T) : size.
+Definition typing_size `{checker_flags} {Σ Δ Γ t T} (d : Σ ;;; Δ ;;; Γ |- t : T) : size.
 Proof.
-  revert Σ Γ t T d.
-  fix typing_size 5.
-  destruct 1 ;
+  revert Σ Δ Γ t T d.
+  fix typing_size 6.
+  pose (wf_size Σ Δ Γ (w : wf_named Σ Δ) (w' : wf_local Σ Δ Γ) := 
+    Nat.max (All_named_env_size (typing_size Σ) Δ w)
+            (All_local_env_size (typing_size Σ Δ) Γ w')).
+  destruct 1;
     repeat match goal with
-           | H : typing _ _ _ _ |- _ => apply typing_size in H
-           end;
-    match goal with
-    | H : All2 _ _ _ |- _ => idtac
-    | H : All2i _ _ _ _ |- _ => idtac
-    | H : All_local_env _ _ |- _ => idtac
-    | H : All _ _ |- _ => idtac
-    | H : Alli _ _ _ |- _ => idtac
-    | H : typing_spine _ _ _ _ _ |- _ => idtac
-    | H : _ + _ |- _ => idtac
-    | H : lift_typing0 _ _ |- _ => idtac
-    | H1 : size, H2 : size, H3 : size |- _ => exact (S (Nat.max H1 (Nat.max H2 H3)))
-    | H1 : size, H2 : size |- _ => exact (S (Nat.max H1 H2))
-    | H1 : size |- _  => exact (S H1)
-    | _ => exact 1
-    end.
-  - exact (S (All_local_env_size (typing_size _) _ a)).
-  - exact (S (All_local_env_size (typing_size _) _ a)).
-  - exact (S (Nat.max d (lift_typing_size (typing_size _ _) _ l))).
-  - exact (S (Nat.max d (lift_typing_size (typing_size _ _) _ l))).
-  - exact (S (Nat.max d (lift_typing_size (typing_size _ _) _ l))).
-  - exact (S (Nat.max d (typing_spine_size typing_size _ _ _ _ _ t0))).
-  - exact (S (S (All_local_env_size (typing_size _) _ a))).
-  - exact (S (S (All_local_env_size (typing_size _) _ a))).
-  - exact (S (S (All_local_env_size (typing_size _) _ a))).
+           | H : typing _ _ _ _ _ |- _ => apply typing_size in H
+           end.
+  - exact (S (wf_size Σ Δ Γ a a0)).
+  - exact (S (wf_size Σ Δ Γ a a0)).
+  - exact (S (wf_size Σ Δ Γ a a0)). 
+  - exact (S (Nat.max d1 d2)).
+  - exact (S (Nat.max d (lift_typing_size (typing_size _ _ _) _ l))).
+  - exact (S (Nat.max d (lift_typing_size (typing_size _ _ _) _ l))).
+  - exact (S (Nat.max d (lift_typing_size (typing_size _ _ _) _ l))).
+  - exact (S (Nat.max d (typing_spine_size typing_size _ _ _ _ _ _ t0))).
+  - exact (S (S (wf_size Σ Δ Γ a a0))).
+  - exact (S (S (wf_size Σ Δ Γ a a0))).
+  - exact (S (S (wf_size Σ Δ Γ a a0))).
   - exact (S (Nat.max d1 (Nat.max d2
     (Nat.max (ctx_inst_size _ typing_size c1)
-      (all2i_size _ (fun _ x y p => Nat.max (typing_size _ _ _ _ p.1.2) (typing_size _ _ _ _ p.2)) a0))))).
+      (all2i_size _ (fun _ x y p => Nat.max (typing_size _ _ _ _ _ p.1.2) (typing_size _ _ _ _ _ p.2)) a0))))).
+  - exact (S d). 
   - exact (S (Nat.max
-      (Nat.max (All_local_env_size (typing_size _) _ a) (all_size _ (fun x p => on_def_type_size (typing_size Σ) _ _ p) a0))
-      (all_size (on_def_body (lift_typing typing _) _ _) (fun x p => on_def_body_size (typing_size Σ) _ _ _ p) a1))).
+      (Nat.max (wf_size Σ Δ Γ a a0) (all_size _ (fun x p => on_def_type_size (typing_size Σ _) _ _ p) a1))
+      (all_size (on_def_body (lift_typing1 (typing Σ Δ)) _ _) (fun x p => on_def_body_size (typing_size Σ Δ) _ _ _ p) a2))).
   - exact (S (Nat.max
-      (Nat.max (All_local_env_size (typing_size _) _ a) (all_size _ (fun x p => on_def_type_size (typing_size Σ) _ _ p) a0))
-      (all_size (on_def_body (lift_typing typing _) _ _) (fun x p => on_def_body_size (typing_size Σ) _ _ _ p) a1))).
-  - exact (S (All_local_env_size (typing_size _) _ a)).
-  - exact (S (All_local_env_size (typing_size _) _ a)).
-  - exact (S (All_local_env_size (typing_size _) _ a)).
-  - exact (S (Nat.max (All_local_env_size (typing_size _) _ a) (Nat.max d2 (Nat.max d3 (all_size _ (fun t p => typing_size Σ Γ t ty p) a0))))).
+      (Nat.max (wf_size Σ Δ Γ a a0) (all_size _ (fun x p => on_def_type_size (typing_size Σ _) _ _ p) a1))
+      (all_size (on_def_body (lift_typing1 (typing Σ Δ)) _ _) (fun x p => on_def_body_size (typing_size Σ Δ) _ _ _ p) a2))).
+  - exact (S (wf_size Σ Δ Γ a a0)).
+  - exact (S (wf_size Σ Δ Γ a a0)).
+  - exact (S (wf_size Σ Δ Γ a a0)).
+  - exact (S (Nat.max (wf_size Σ Δ Γ a a0) (Nat.max d2 (Nat.max d3 (all_size _ (fun t p => typing_size Σ Δ Γ t ty p) a1))))).
+  - exact (S (Nat.max d1 d2)).  
 Defined.
 
-Lemma typing_size_pos `{checker_flags} {Σ Γ t T} (d : Σ ;;; Γ |- t : T) : typing_size d > 0.
+Lemma typing_size_pos `{checker_flags} {Σ Δ Γ t T} (d : Σ ;;; Δ ;;; Γ |- t : T) : typing_size d > 0.
 Proof.
   induction d; simpl; try lia.
 Qed.
@@ -1063,79 +1069,115 @@ Definition globenv_size (Σ : global_env) : size :=
 
 Arguments lexprod [A B].
 
-Definition wf `{checker_flags} Σ := on_global_env cumul_gen (lift_typing typing) Σ.
-Definition wf_ext `{checker_flags} := on_global_env_ext cumul_gen (lift_typing typing).
+Definition wf `{checker_flags} Σ := on_global_env cumul_gen (lift_typing3 typing) Σ.
+Definition wf_ext `{checker_flags} := on_global_env_ext cumul_gen (lift_typing3 typing).
 
-Lemma typing_wf_local `{cf : checker_flags} {Σ} {Γ t T} :
-  Σ ;;; Γ |- t : T -> wf_local Σ Γ.
+Lemma typing_wf_local `{cf : checker_flags} {Σ} {Δ Γ t T} :
+  Σ ;;; Δ ;;; Γ |- t : T -> wf_local Σ Δ Γ.
 Proof.
-  revert Σ Γ t T.
-  fix f 5.
+  revert Σ Δ Γ t T.
+  fix f 6.
   destruct 1; eauto.
-  all: exact (f _ _ _ _ l.2.π2.1).
+  all: exact (f _ _ _ _ _ l.2.π2.1).
 Defined.
 #[global] Hint Resolve typing_wf_local : wf.
 
-Lemma type_Prop `{checker_flags} Σ :
-  Σ ;;; [] |- tSort sProp : tSort Sort.type1.
-  change (  Σ ;;; [] |- tSort (sProp) : tSort Sort.type1);
-  constructor;auto. constructor. constructor.
-Defined.
-
-Lemma type_Prop_wf `{checker_flags} Σ Γ :
-  wf_local Σ Γ ->
-  Σ ;;; Γ |- tSort sProp : tSort Sort.type1.
+Lemma typing_wf_named `{cf : checker_flags} {Σ} {Δ Γ t T} :
+  Σ ;;; Δ ;;; Γ |- t : T -> wf_named Σ Δ.
 Proof.
-  constructor;auto. constructor.
+  revert Σ Δ Γ t T.
+  fix f 6.
+  destruct 1; eauto.
+  all: exact (f _ _ _ _ _ l.2.π2.1).
+Defined.
+#[global] Hint Resolve typing_wf_named : wf.
+
+Lemma type_Prop `{checker_flags} Σ :
+  Σ ;;; [] ;;; [] |- tSort sProp : tSort Sort.type1.
+  change (  Σ ;;; [] ;;; [] |- tSort (sProp) : tSort Sort.type1);
+  constructor ; auto ; constructor.
 Defined.
 
-Definition env_prop `{checker_flags} (P : forall Σ Γ t T, Type) (Pj : forall Σ Γ j, Type) (PΓ : forall Σ Γ (wfΓ : wf_local Σ Γ), Type):=
-  forall (Σ : global_env_ext) (wfΣ : wf Σ) Γ (wfΓ : wf_local Σ Γ) t T (ty : Σ ;;; Γ |- t : T),
-    on_global_env cumul_gen Pj Σ * (PΓ Σ Γ (typing_wf_local ty) * P Σ Γ t T).
+Lemma typing_size_Prop `{checker_flags} Σ :
+  typing_size (type_Prop Σ) = 1.
+Proof.
+  simpl. unfold All_local_env_size. simpl. reflexivity.
+Qed.
 
-Lemma env_prop_typing `{checker_flags} {P Pj PΓ} : env_prop P Pj PΓ ->
-  forall (Σ : global_env_ext) (wfΣ : wf Σ) (Γ : context) (wfΓ : wf_local Σ Γ) (t T : term),
-    Σ ;;; Γ |- t : T -> P Σ Γ t T.
+Lemma type_Prop_wf `{checker_flags} Σ Δ Γ :
+  wf_named Σ Δ ->
+  wf_local Σ Δ Γ ->
+  Σ ;;; Δ ;;; Γ |- tSort sProp : tSort Sort.type1.
+Proof.
+  constructor ; auto ; constructor.
+Defined.
+
+Definition env_prop `{checker_flags} (P : forall Σ Δ Γ t T, Type) (Pj : forall Σ Δ Γ j, Type) 
+  (PΔ : forall Σ Δ (wfΔ : wf_named Σ Δ), Type)  (PΓ : forall Σ Δ (wfΔ : wf_named Σ Δ) Γ (wfΓ : wf_local Σ Δ Γ), Type) :=
+  forall (Σ : global_env_ext) (wfΣ : wf Σ) Δ Γ t T (ty : Σ ;;; Δ ;;; Γ |- t : T),
+    on_global_env cumul_gen Pj Σ * (PΔ Σ Δ (typing_wf_named ty) * PΓ Σ Δ (typing_wf_named ty) Γ (typing_wf_local ty) * P Σ Δ Γ t T).
+
+Lemma env_prop_typing `{checker_flags} {P Pj PΔ PΓ} : env_prop P Pj PΔ PΓ ->
+  forall (Σ : global_env_ext) (wfΣ : wf Σ) (Δ : named_context) (Γ : context) (t T : term),
+    Σ ;;; Δ ;;; Γ |- t : T -> P Σ Δ Γ t T.
 Proof. intros. now apply X. Qed.
 
-Lemma env_prop_wf_local `{checker_flags} {P Pj PΓ} : env_prop P Pj PΓ ->
-  forall (Σ : global_env_ext) (wfΣ : wf Σ) (Γ : context) (wfΓ : wf_local Σ Γ), PΓ Σ Γ wfΓ.
-Proof. intros. red in X. now apply (X _ wfΣ _ wfΓ _ _ (type_Prop_wf Σ Γ wfΓ)). Qed.
+Lemma env_prop_wf_local `{checker_flags} {P Pj PΔ PΓ} : env_prop P Pj PΔ PΓ ->
+  forall (Σ : global_env_ext) (wfΣ : wf Σ) (Δ : named_context) (wfΔ : wf_named Σ Δ) 
+    (Γ : context) (wfΓ : wf_local Σ Δ Γ), PΓ Σ Δ wfΔ Γ wfΓ.
+Proof. intros. red in X. now apply (X Σ wfΣ Δ Γ _ _ (type_Prop_wf Σ Δ Γ _ _)). Qed.
 
-Lemma env_prop_sigma `{checker_flags} {P Pj PΓ} : env_prop P Pj PΓ ->
+Lemma env_prop_sigma `{checker_flags} {P Pj PΔ PΓ} : env_prop P Pj PΔ PΓ ->
   forall Σ (wfΣ : wf Σ), on_global_env cumul_gen Pj Σ.
 Proof.
   intros. eapply (X (empty_ext Σ)).
-  apply wfΣ. constructor.
-  apply type_Prop.
+  - apply wfΣ.
+  - apply type_Prop.
 Defined.
 
-Lemma wf_local_app_l `{checker_flags} Σ (Γ Γ' : context) : wf_local Σ (Γ ,,, Γ') -> wf_local Σ Γ.
+Lemma wf_local_app_l `{checker_flags} Σ Δ (Γ Γ' : context) : wf_local Σ Δ (Γ ,,, Γ') -> wf_local Σ Δ Γ.
 Proof.
-  induction Γ'. auto.
-  simpl. intros H'; inv H'; eauto.
+  induction Γ'.
+  - auto.
+  - simpl. intros H'. apply IHΓ'. now inv H'.
 Defined.
 #[global] Hint Immediate wf_local_app_l : wf.
 
-Lemma typing_wf_local_size `{cf : checker_flags} {Σ} {Γ t T}
-      (d :Σ ;;; Γ |- t : T) :
-  All_local_env_size (@typing_size _ _) _ (typing_wf_local d) < typing_size d.
+Lemma wf_named_app_l `{checker_flags} Σ Δ Δ' : wf_named Σ (Δ ,,, Δ') -> wf_named Σ Δ.
 Proof.
-  revert Σ Γ t T d. fix f 5.
-  induction d; simpl;
-  change (fun Γ t T (Hty : Σ;;; Γ |- t : T) => typing_size Hty) with (@typing_size cf Σ); try lia.
-  1-3: pose proof (f _ _ _ _ l.2.π2.1); unfold lift_sorting_size; cbn in *; try lia.
+  induction Δ'.
+  - auto.
+  - simpl. intros H'. apply IHΔ'. now inv H'.
+Defined.
+#[global] Hint Immediate wf_named_app_l : wf.  
 
+Lemma typing_wf_local_size `{cf : checker_flags} {Σ} {Δ Γ t T}
+      (d : Σ ;;; Δ ;;; Γ |- t : T) :
+  All_local_env_size (@typing_size cf Σ Δ) Γ (typing_wf_local d) < typing_size d.
+Proof.
+  revert Σ Δ Γ t T d. fix f 6.
+  induction d; simpl;
+  change (fun Γ t T (Hty : Σ ;;; Δ ;;; Γ |- t : T) => typing_size Hty) with (@typing_size cf Σ); try lia.
+  1-3: pose proof (f _ _ _ _ _ l.2.π2.1); unfold lift_sorting_size; cbn in *; try lia.
 Qed.
 
-Lemma wf_local_inv `{checker_flags} {Σ Γ'} (w : wf_local Σ Γ') :
+Lemma typing_wf_named_size `{cf : checker_flags} {Σ} {Δ Γ t T}
+      (d : Σ ;;; Δ ;;; Γ |- t : T) :
+  All_named_env_size (@typing_size cf Σ) Δ (typing_wf_named d) < typing_size d.
+Proof.
+  revert Σ Δ Γ t T d. fix f 6.
+  induction d; simpl;
+  change (fun Γ t T (Hty : Σ ;;; Δ ;;; Γ |- t : T) => typing_size Hty) with (@typing_size cf Σ); try lia.
+Qed.
+
+Lemma wf_local_inv `{checker_flags} {Σ Δ Γ'} (w : wf_local Σ Δ Γ') :
   forall d Γ,
     Γ' = d :: Γ ->
-    ∑ (w' : wf_local Σ Γ) u,
-      { ty : lift_typing1 (typing Σ) Γ (Judge d.(decl_body) d.(decl_type) (Some u)) |
-            All_local_env_size (@typing_size _ Σ) _ w' <
-            All_local_env_size (@typing_size _ _) _ w /\
-            lift_typing_size (@typing_size _ _ _) _ ty <= All_local_env_size (@typing_size _ _) _ w }.
+    ∑ (w' : wf_local Σ Δ Γ) u,
+      { ty : lift_typing1 (typing Σ Δ) Γ (Judge d.(decl_body) d.(decl_type) (Some u)) |
+            All_local_env_size (@typing_size _ Σ Δ) _ w' <
+            All_local_env_size (@typing_size _ Σ Δ) _ w /\
+            lift_typing_size (@typing_size _ Σ Δ Γ) _ ty <= All_local_env_size (@typing_size _ _ _) _ w }.
 Proof.
   intros d Γ ->.
   depelim w; cbn.
@@ -1147,6 +1189,28 @@ Proof.
   all: try lia.
 Qed.
 
+Lemma wf_named_inv `{checker_flags} {Σ Δ' id} (w : wf_named Σ Δ') :
+  forall d Δ,
+    Δ' = (id, d) :: Δ ->
+    ∑ (w' : wf_named Σ Δ) u,
+      { ty : lift_typing0 (typing Σ Δ []) (Judge d.(decl_body) d.(decl_type) (Some u)) |
+            All_named_env_size (@typing_size _ Σ) _ w' <
+            All_named_env_size (@typing_size _ Σ) _ w /\
+            lift_typing_size (@typing_size _ Σ Δ []) _ ty <= All_named_env_size (@typing_size _ _) _ w }.
+Proof.
+  intros d Δ ->.
+  depelim w; cbn.
+  all: exists w, l.2.π1, (lift_sorting_extract l).
+  all: pose proof (typing_size_pos l.2.π2.1).
+  2: pose proof (typing_size_pos l.1).
+  all: simpl in *.
+  all: simpl; split.
+  all: try lia.
+Qed.
+
+(*Lemma typing_nctx_inv Σ Δ Γ id na ta t T :
+  Σ ;;; Δ ,, (id, vass na ta) ;;; Γ |- t : T ->
+  Σ ;;; Δ *)
 
 (** *** An induction principle ensuring the Σ declarations enjoy the same properties.
     Also theads the well-formedness of the local context and the induction principle for it,
@@ -1154,219 +1218,258 @@ Qed.
     on typing judgments in application spines, fix and cofix blocks.
  *)
 
-Inductive Forall_typing_spine `{checker_flags} Σ Γ (P : term -> term -> Type) :
-  forall (T : term) (t : list term) (U : term), typing_spine Σ Γ T t U -> Type :=
-| Forall_type_spine_nil T : Forall_typing_spine Σ Γ P T [] T (type_spine_nil Σ Γ T)
+Inductive Forall_typing_spine `{checker_flags} Σ Δ Γ (P : term -> term -> Type) :
+  forall (T : term) (t : list term) (U : term), typing_spine Σ Δ Γ T t U -> Type :=
+| Forall_type_spine_nil T : Forall_typing_spine Σ Δ Γ P T [] T (type_spine_nil Σ Δ Γ T)
 | Forall_type_spine_cons hd tl na A B s T B' tls
-   (typrod : Σ ;;; Γ |- tProd na A B : tSort s)
-   (cumul : Σ ;;; Γ |- T <= tProd na A B) (ty : Σ ;;; Γ |- hd : A) :
-    P (tProd na A B) (tSort s) -> P hd A -> Forall_typing_spine Σ Γ P (B {0 := hd}) tl B' tls ->
-    Forall_typing_spine Σ Γ P T (hd :: tl) B'
-      (type_spine_cons Σ Γ hd tl na A B s T B' typrod cumul ty tls).
+   (typrod : Σ ;;; Δ ;;; Γ |- tProd na A B : tSort s)
+   (cumul : Σ ;;; Δ ;;; Γ |- T <= tProd na A B) (ty : Σ ;;; Δ ;;; Γ |- hd : A) :
+    P (tProd na A B) (tSort s) -> P hd A -> Forall_typing_spine Σ Δ Γ P (B {0 := hd}) tl B' tls ->
+    Forall_typing_spine Σ Δ Γ P T (hd :: tl) B'
+      (type_spine_cons Σ Δ Γ hd tl na A B s T B' typrod cumul ty tls).
 
 Implicit Types (Σ : global_env_ext).
 
 Lemma typing_ind_env `{cf : checker_flags} :
-  forall (P : global_env_ext -> context -> term -> term -> Type)
-         (Pj : global_env_ext -> context -> judgment -> Type)
-         (Pdecl := fun Σ Γ wfΓ t T tyT => P Σ Γ t T)
-         (PΓ : forall Σ Γ, wf_local Σ Γ -> Type),
+  forall (P : global_env_ext -> named_context -> context -> term -> term -> Type)
+         (Pj : global_env_ext -> named_context -> context -> judgment -> Type)
+         (Pdecl := fun Σ Δ (wfΔ : wf_named Σ Δ) Γ (wfΓ : wf_local Σ Δ Γ) t T tyT => P Σ Δ Γ t T)
+         (PΔ : forall Σ Δ (_ : wf_named Σ Δ), Type)
+         (PΓ : forall Σ Δ (_ : wf_named Σ Δ) Γ (_ : wf_local Σ Δ Γ), Type),
 
-    (forall Σ (wfΣ : wf Σ) (Γ : context) (* (wfΓ : wf_local Σ Γ) *) j,
-      lift_typing_conj (typing Σ) (P Σ) Γ j -> Pj Σ Γ j) ->
+    (forall Σ (wfΣ : wf Σ) (Δ : named_context) (* (wfΔ : wf_named Σ Δ) *) (Γ : context) (* (wfΓ : wf_local Σ Δ Γ) *) j,
+      lift_typing_conj1 (typing Σ Δ) (P Σ Δ) Γ j -> Pj Σ Δ Γ j) ->
 
-    (forall Σ (wfΣ : wf Σ) (Γ : context) (wfΓ : wf_local Σ Γ),
-      All_local_env_over (typing Σ) (Pdecl Σ) Γ wfΓ -> All_local_env (Pj Σ) Γ -> PΓ Σ Γ wfΓ) ->
+    (forall Σ (wfΣ : wf Σ) (Δ : named_context) (wfΔ : wf_named Σ Δ),
+      All_named_env_over (typing Σ) (fun Δ Γ wfΔ t T tyT => P Σ Δ Γ t T) Δ wfΔ -> 
+      All_named_env (Pj Σ) Δ ->
+      PΔ Σ Δ wfΔ) ->
 
-    (forall Σ (wfΣ : wf Σ) (Γ : context) (wfΓ : wf_local Σ Γ) (n : nat) decl,
-        nth_error Γ n = Some decl ->
-        PΓ Σ Γ wfΓ ->
-        P Σ Γ (tRel n) (lift0 (S n) decl.(decl_type))) ->
-    (forall Σ (wfΣ : wf Σ) (Γ : context) (wfΓ : wf_local Σ Γ) (u : sort),
-      PΓ Σ Γ wfΓ ->
+    (forall Σ (wfΣ : wf Σ) (Δ : named_context) (wfΔ : wf_named Σ Δ) (Γ : context) (wfΓ : wf_local Σ Δ Γ),
+      All_named_env_over (typing Σ) (fun Δ Γ wfΔ t T tyT => P Σ Δ Γ t T) Δ wfΔ -> All_named_env (Pj Σ) Δ ->
+      All_local_env_over (typing Σ Δ) (Pdecl Σ Δ wfΔ) Γ wfΓ -> All_local_env (Pj Σ Δ) Γ -> PΓ Σ Δ wfΔ Γ wfΓ) ->
+
+    (forall Σ (wfΣ : wf Σ) (Δ : named_context) (wfΔ : wf_named Σ Δ) (Γ : context) (wfΓ : wf_local Σ Δ Γ) (n : nat) decl,
+      nth_error Γ n = Some decl ->
+      PΔ Σ Δ wfΔ ->
+      PΓ Σ Δ wfΔ Γ wfΓ ->
+      P Σ Δ Γ (tRel n) (lift0 (S n) decl.(decl_type))) ->
+
+    (forall Σ (wfΣ : wf Σ) (Δ : named_context) (wfΔ : wf_named Σ Δ) (Γ : context) (wfΓ : wf_local Σ Δ Γ) (id : ident) decl,
+      nctx_lookup Δ id = Some decl ->
+      PΔ Σ Δ wfΔ ->
+      PΓ Σ Δ wfΔ Γ wfΓ ->
+      P Σ Δ Γ (tVar id) decl.(decl_type)) ->
+
+    (forall Σ (wfΣ : wf Σ) (Δ : named_context) (wfΔ : wf_named Σ Δ) (Γ : context) (wfΓ : wf_local Σ Δ Γ) (u : sort),
+      PΔ Σ Δ wfΔ ->
+      PΓ Σ Δ wfΔ Γ wfΓ ->
       wf_sort Σ u ->
-      P Σ Γ (tSort u) (tSort (Sort.super u))) ->
+      P Σ Δ Γ (tSort u) (tSort (Sort.super u))) ->
 
-    (forall Σ (wfΣ : wf Σ) (Γ : context) (wfΓ : wf_local Σ Γ) (c : term) (k : cast_kind)
-            (t : term) (s : sort),
-        Σ ;;; Γ |- t : tSort s -> P Σ Γ t (tSort s) -> Σ ;;; Γ |- c : t -> P Σ Γ c t -> P Σ Γ (tCast c k t) t) ->
+    (forall Σ (wfΣ : wf Σ) (Δ : named_context) (wfΔ : wf_named Σ Δ) (Γ : context) (wfΓ : wf_local Σ Δ Γ) 
+            (c : term) (k : cast_kind) (t : term) (s : sort),
+        Σ ;;; Δ ;;; Γ |- t : tSort s -> P Σ Δ Γ t (tSort s) -> 
+        Σ ;;; Δ ;;; Γ |- c : t -> P Σ Δ Γ c t -> 
+        P Σ Δ Γ (tCast c k t) t) ->
 
-    (forall Σ (wfΣ : wf Σ) (Γ : context) (wfΓ : wf_local Σ Γ) (na : aname) (t b : term) (s1 s2 : sort),
-        PΓ Σ Γ wfΓ ->
-        lift_typing typing Σ Γ (j_vass_s na t s1) ->
-        Pj Σ Γ (j_vass_s na t s1) ->
-        Σ ;;; Γ,, vass na t |- b : tSort s2 ->
-        P Σ (Γ,, vass na t) b (tSort s2) -> P Σ Γ (tProd na t b) (tSort (Sort.sort_of_product s1 s2))) ->
+    (forall Σ (wfΣ : wf Σ) (Δ : named_context) (wfΔ : wf_named Σ Δ) (Γ : context) (wfΓ : wf_local Σ Δ Γ) (na : aname) 
+            (t b : term) (s1 s2 : sort),
+        PΔ Σ Δ wfΔ ->
+        PΓ Σ Δ wfΔ Γ wfΓ ->
+        lift_typing3 typing Σ Δ Γ (j_vass_s na t s1) ->
+        Pj Σ Δ Γ (j_vass_s na t s1) ->
+        Σ ;;; Δ ;;; Γ ,, vass na t |- b : tSort s2 ->
+        P Σ Δ (Γ ,, vass na t) b (tSort s2) -> P Σ Δ Γ (tProd na t b) (tSort (Sort.sort_of_product s1 s2))) ->
 
-    (forall Σ (wfΣ : wf Σ) (Γ : context) (wfΓ : wf_local Σ Γ) (na : aname) (t b : term) (bty : term),
-        PΓ Σ Γ wfΓ ->
-        lift_typing typing Σ Γ (j_vass na t) ->
-        Pj Σ Γ (j_vass na t) ->
-        Σ ;;; Γ,, vass na t |- b : bty -> P Σ (Γ,, vass na t) b bty -> P Σ Γ (tLambda na t b) (tProd na t bty)) ->
+    (forall Σ (wfΣ : wf Σ)(Δ : named_context) (wfΔ : wf_named Σ Δ) (Γ : context) (wfΓ : wf_local Σ Δ Γ) 
+            (na : aname) (t b : term) (bty : term),
+        PΔ Σ Δ wfΔ ->
+        PΓ Σ Δ wfΔ Γ wfΓ ->
+        lift_typing3 typing Σ Δ Γ (j_vass na t) ->
+        Pj Σ Δ Γ (j_vass na t) ->
+        Σ ;;; Δ ;;; Γ ,, vass na t |- b : bty -> P Σ Δ (Γ ,, vass na t) b bty -> P Σ Δ Γ (tLambda na t b) (tProd na t bty)) ->
 
-    (forall Σ (wfΣ : wf Σ) (Γ : context) (wfΓ : wf_local Σ Γ) (na : aname) (b b_ty b' b'_ty : term),
-        PΓ Σ Γ wfΓ ->
-        lift_typing typing Σ Γ (j_vdef na b b_ty) ->
-        Pj Σ Γ (j_vdef na b b_ty) ->
-        Σ ;;; Γ,, vdef na b b_ty |- b' : b'_ty ->
-        P Σ (Γ,, vdef na b b_ty) b' b'_ty -> P Σ Γ (tLetIn na b b_ty b') (tLetIn na b b_ty b'_ty)) ->
+    (forall Σ (wfΣ : wf Σ) (Δ : named_context) (wfΔ : wf_named Σ Δ) (Γ : context) (wfΓ : wf_local Σ Δ Γ) 
+            (na : aname) (b b_ty b' b'_ty : term),
+        PΔ Σ Δ wfΔ ->
+        PΓ Σ Δ wfΔ Γ wfΓ ->
+        lift_typing3 typing Σ Δ Γ (j_vdef na b b_ty) ->
+        Pj Σ Δ Γ (j_vdef na b b_ty) ->
+        Σ ;;; Δ ;;; Γ ,, vdef na b b_ty |- b' : b'_ty ->
+        P Σ Δ (Γ ,, vdef na b b_ty) b' b'_ty -> P Σ Δ Γ (tLetIn na b b_ty b') (tLetIn na b b_ty b'_ty)) ->
 
-    (forall Σ (wfΣ : wf Σ) (Γ : context) (wfΓ : wf_local Σ Γ) (t : term) (l : list term) (t_ty t' : term),
-        Σ ;;; Γ |- t : t_ty -> P Σ Γ t t_ty ->
+    (forall Σ (wfΣ : wf Σ) (Δ : named_context) (wfΔ : wf_named Σ Δ) (Γ : context) (wfΓ : wf_local Σ Δ Γ) 
+            (t : term) (l : list term) (t_ty t' : term),
+        Σ ;;; Δ ;;; Γ |- t : t_ty -> P Σ Δ Γ t t_ty ->
         isApp t = false -> l <> [] ->
-        forall (s : typing_spine Σ Γ t_ty l t'),
-        Forall_typing_spine Σ Γ (fun t T => P Σ Γ t T) t_ty l t' s ->
-        P Σ Γ (tApp t l) t') ->
+        forall (s : typing_spine Σ Δ Γ t_ty l t'),
+        Forall_typing_spine Σ Δ Γ (fun t T => P Σ Δ Γ t T) t_ty l t' s ->
+        P Σ Δ Γ (tApp t l) t') ->
 
-    (forall Σ (wfΣ : wf Σ) (Γ : context) (wfΓ : wf_local Σ Γ) cst u (decl : constant_body),
+    (forall Σ (wfΣ : wf Σ) (Δ : named_context) (wfΔ : wf_named Σ Δ) (Γ : context) (wfΓ : wf_local Σ Δ Γ) 
+            cst u (decl : constant_body),
         on_global_env cumul_gen Pj Σ.1 ->
-        PΓ Σ Γ wfΓ ->
+        PΔ Σ Δ wfΔ ->
+        PΓ Σ Δ wfΔ Γ wfΓ ->
         declared_constant Σ.1 cst decl ->
         consistent_instance_ext Σ decl.(cst_universes) u ->
-        P Σ Γ (tConst cst u) (subst_instance u (cst_type decl))) ->
+        P Σ Δ Γ (tConst cst u) (subst_instance u (cst_type decl))) ->
 
-    (forall Σ (wfΣ : wf Σ) (Γ : context) (wfΓ : wf_local Σ Γ) (ind : inductive) u
+    (forall Σ (wfΣ : wf Σ) (Δ : named_context) (wfΔ : wf_named Σ Δ) (Γ : context) (wfΓ : wf_local Σ Δ Γ) (ind : inductive) u
           mdecl idecl (isdecl : declared_inductive Σ.1 ind mdecl idecl),
         on_global_env cumul_gen Pj Σ.1 ->
-        PΓ Σ Γ wfΓ ->
+        PΔ Σ Δ wfΔ ->
+        PΓ Σ Δ wfΔ Γ wfΓ ->
         consistent_instance_ext Σ mdecl.(ind_universes) u ->
-        P Σ Γ (tInd ind u) (subst_instance u (ind_type idecl))) ->
+        P Σ Δ Γ (tInd ind u) (subst_instance u (ind_type idecl))) ->
 
-    (forall Σ (wfΣ : wf Σ) (Γ : context) (wfΓ : wf_local Σ Γ) (ind : inductive) (i : nat) u
+    (forall Σ (wfΣ : wf Σ) (Δ : named_context) (wfΔ : wf_named Σ Δ) (Γ : context) (wfΓ : wf_local Σ Δ Γ) (ind : inductive) (i : nat) u
             mdecl idecl cdecl (isdecl : declared_constructor Σ.1 (ind, i) mdecl idecl cdecl),
         on_global_env cumul_gen Pj Σ.1 ->
-        PΓ Σ Γ wfΓ ->
+        PΔ Σ Δ wfΔ ->
+        PΓ Σ Δ wfΔ Γ wfΓ ->
         consistent_instance_ext Σ mdecl.(ind_universes) u ->
-        P Σ Γ (tConstruct ind i u) (type_of_constructor mdecl cdecl (ind, i) u)) ->
+        P Σ Δ Γ (tConstruct ind i u) (type_of_constructor mdecl cdecl (ind, i) u)) ->
 
-     (forall (Σ : global_env_ext) (wfΣ : wf Σ) (Γ : context) (wfΓ : wf_local Σ Γ),
+     (forall (Σ : global_env_ext) (wfΣ : wf Σ) (Δ : named_context) (wfΔ : wf_named Σ Δ) (Γ : context) (wfΓ : wf_local Σ Δ Γ),
       forall (ci : case_info) p c brs indices ps mdecl idecl
         (isdecl : declared_inductive Σ.1 ci.(ci_ind) mdecl idecl),
         on_global_env cumul_gen Pj Σ.1 ->
-        PΓ Σ Γ wfΓ ->
+        PΔ Σ Δ wfΔ ->
+        PΓ Σ Δ wfΔ Γ wfΓ ->
         mdecl.(ind_npars) = ci.(ci_npar) ->
         wf_nactx p.(pcontext) (ind_predicate_context ci.(ci_ind) mdecl idecl) ->
         context_assumptions mdecl.(ind_params) = #|p.(pparams)| ->
         consistent_instance_ext Σ (ind_universes mdecl) p.(puinst) ->
         let predctx := case_predicate_context ci.(ci_ind) mdecl idecl p in
-        ctx_inst (Prop_conj typing P Σ) Γ (p.(pparams) ++ indices)
+        ctx_inst ((Prop_conj typing P Σ) Δ) Γ (p.(pparams) ++ indices)
         (List.rev (ind_params mdecl ,,, ind_indices idecl : context)@[p.(puinst)]) ->
-        forall pret : Σ ;;; Γ ,,, predctx |- p.(preturn) : tSort ps,
-        P Σ (Γ ,,, predctx) p.(preturn) (tSort ps) ->
-        PΓ Σ (Γ ,,, predctx) (typing_wf_local pret) ->
+        forall pret : Σ ;;; Δ ;;; Γ ,,, predctx |- p.(preturn) : tSort ps,
+        P Σ Δ (Γ ,,, predctx) p.(preturn) (tSort ps) ->
+        PΓ Σ Δ (typing_wf_named pret) (Γ ,,, predctx) (typing_wf_local pret) ->
         is_allowed_elimination Σ idecl.(ind_kelim) ps ->
-        Σ ;;; Γ |- c : mkApps (tInd ci.(ci_ind) p.(puinst)) (p.(pparams) ++ indices) ->
-        P Σ Γ c (mkApps (tInd ci.(ci_ind) p.(puinst)) (p.(pparams) ++ indices)) ->
+        Σ ;;; Δ ;;; Γ |- c : mkApps (tInd ci.(ci_ind) p.(puinst)) (p.(pparams) ++ indices) ->
+        P Σ Δ Γ c (mkApps (tInd ci.(ci_ind) p.(puinst)) (p.(pparams) ++ indices)) ->
         isCoFinite mdecl.(ind_finite) = false ->
         let ptm := it_mkLambda_or_LetIn predctx p.(preturn) in
         All2i (fun i cdecl br =>
           let brctxty := case_branch_type ci.(ci_ind) mdecl p ptm i cdecl br in
           wf_nactx br.(bcontext) (cstr_branch_context ci.(ci_ind) mdecl cdecl) *
-          Prop_conj typing P Σ (Γ ,,, brctxty.1) br.(bbody) brctxty.2 *
-          Prop_conj typing P Σ (Γ ,,, brctxty.1) brctxty.2 (tSort ps))
+          Prop_conj typing P Σ Δ (Γ ,,, brctxty.1) br.(bbody) brctxty.2 *
+          Prop_conj typing P Σ Δ (Γ ,,, brctxty.1) brctxty.2 (tSort ps))
           0 idecl.(ind_ctors) brs ->
-        P Σ Γ (tCase ci p c brs) (mkApps ptm (indices ++ [c]))) ->
+        P Σ Δ Γ (tCase ci p c brs) (mkApps ptm (indices ++ [c]))) ->
 
-    (forall Σ (wfΣ : wf Σ) (Γ : context) (wfΓ : wf_local Σ Γ) (p : projection) (c : term) u
+    (forall Σ (wfΣ : wf Σ) (Δ : named_context) (wfΔ : wf_named Σ Δ) (Γ : context) (wfΓ : wf_local Σ Δ Γ) (p : projection) (c : term) u
           mdecl idecl cdecl pdecl (isdecl : declared_projection Σ.1 p mdecl idecl cdecl pdecl) args,
         on_global_env cumul_gen Pj Σ.1 ->
-        PΓ Σ Γ wfΓ ->
-        Σ ;;; Γ |- c : mkApps (tInd p.(proj_ind) u) args ->
-        P Σ Γ c (mkApps (tInd p.(proj_ind) u) args) ->
+        PΔ Σ Δ wfΔ ->
+        PΓ Σ Δ wfΔ Γ wfΓ ->
+        Σ ;;; Δ ;;; Γ |- c : mkApps (tInd p.(proj_ind) u) args ->
+        P Σ Δ Γ c (mkApps (tInd p.(proj_ind) u) args) ->
         #|args| = ind_npars mdecl ->
-        P Σ Γ (tProj p c) (subst0 (c :: List.rev args) (subst_instance u pdecl.(proj_type)))) ->
+        P Σ Δ Γ (tProj p c) (subst0 (c :: List.rev args) (subst_instance u pdecl.(proj_type)))) ->
 
-    (forall Σ (wfΣ : wf Σ) (Γ : context) (wfΓ : wf_local Σ Γ) (mfix : list (def term)) (n : nat) decl,
+    (forall Σ (wfΣ : wf Σ) (Δ : named_context) (wfΔ : wf_named Σ Δ) (Γ : context) (wfΓ : wf_local Σ Δ Γ) 
+            (mfix : list (def term)) (n : nat) decl,
         let types := fix_context mfix in
-        fix_guard Σ Γ mfix ->
+        fix_guard Σ Δ Γ mfix ->
         nth_error mfix n = Some decl ->
-        PΓ Σ Γ wfΓ ->
-        All (on_def_type (lift_typing typing Σ) Γ) mfix ->
-        All (on_def_type (Pj Σ) Γ) mfix ->
-        All (on_def_body (lift_typing typing Σ) types Γ) mfix ->
-        All (on_def_body (Pj Σ) types Γ) mfix ->
+        PΔ Σ Δ wfΔ ->
+        PΓ Σ Δ wfΔ Γ wfΓ ->
+        All (on_def_type (lift_typing3 typing Σ Δ) Γ) mfix ->
+        All (on_def_type (Pj Σ Δ) Γ) mfix ->
+        All (on_def_body (lift_typing3 typing Σ Δ) types Γ) mfix ->
+        All (on_def_body (Pj Σ Δ) types Γ) mfix ->
          wf_fixpoint Σ.1 mfix ->
-        P Σ Γ (tFix mfix n) decl.(dtype)) ->
+        P Σ Δ Γ (tFix mfix n) decl.(dtype)) ->
 
-    (forall Σ (wfΣ : wf Σ) (Γ : context) (wfΓ : wf_local Σ Γ) (mfix : list (def term)) (n : nat) decl,
+    (forall Σ (wfΣ : wf Σ) (Δ : named_context) (wfΔ : wf_named Σ Δ) (Γ : context) (wfΓ : wf_local Σ Δ Γ) (mfix : list (def term)) (n : nat) decl,
         let types := fix_context mfix in
-        cofix_guard Σ Γ mfix ->
+        cofix_guard Σ Δ Γ mfix ->
         nth_error mfix n = Some decl ->
-        PΓ Σ Γ wfΓ ->
-        All (on_def_type (lift_typing typing Σ) Γ) mfix ->
-        All (on_def_type (Pj Σ) Γ) mfix ->
-        All (on_def_body (lift_typing typing Σ) types Γ) mfix ->
-        All (on_def_body (Pj Σ) types Γ) mfix ->
+        PΔ Σ Δ wfΔ ->
+        PΓ Σ Δ wfΔ Γ wfΓ ->
+        All (on_def_type (lift_typing3 typing Σ Δ) Γ) mfix ->
+        All (on_def_type (Pj Σ Δ) Γ) mfix ->
+        All (on_def_body (lift_typing3 typing Σ Δ) types Γ) mfix ->
+        All (on_def_body (Pj Σ Δ) types Γ) mfix ->
          wf_cofixpoint Σ.1 mfix ->
-        P Σ Γ (tCoFix mfix n) decl.(dtype)) ->
+        P Σ Δ Γ (tCoFix mfix n) decl.(dtype)) ->
 
-    (forall Σ (wfΣ : wf Σ) (Γ : context) (wfΓ : wf_local Σ Γ) p prim_ty cdecl,
-        PΓ Σ Γ wfΓ ->
+    (forall Σ (wfΣ : wf Σ) (Δ : named_context) (wfΔ : wf_named Σ Δ) (Γ : context) (wfΓ : wf_local Σ Δ Γ) p prim_ty cdecl,
+        PΔ Σ Δ wfΔ ->
+        PΓ Σ Δ wfΔ Γ wfΓ ->
         primitive_constant Σ primInt = Some prim_ty ->
         declared_constant Σ prim_ty cdecl ->
         primitive_invariants primInt cdecl ->
-        P Σ Γ (tInt p) (tConst prim_ty [])) ->
+        P Σ Δ Γ (tInt p) (tConst prim_ty [])) ->
 
-    (forall Σ (wfΣ : wf Σ) (Γ : context) (wfΓ : wf_local Σ Γ) p prim_ty cdecl,
-        PΓ Σ Γ wfΓ ->
+    (forall Σ (wfΣ : wf Σ) (Δ : named_context) (wfΔ : wf_named Σ Δ) (Γ : context) (wfΓ : wf_local Σ Δ Γ) p prim_ty cdecl,
+        PΔ Σ Δ wfΔ ->
+        PΓ Σ Δ wfΔ Γ wfΓ ->
         primitive_constant Σ primFloat = Some prim_ty ->
         declared_constant Σ prim_ty cdecl ->
         primitive_invariants primFloat cdecl ->
-        P Σ Γ (tFloat p) (tConst prim_ty [])) ->
+        P Σ Δ Γ (tFloat p) (tConst prim_ty [])) ->
 
-    (forall Σ (wfΣ : wf Σ) (Γ : context) (wfΓ : wf_local Σ Γ) p prim_ty cdecl,
-        PΓ Σ Γ wfΓ ->
+    (forall Σ (wfΣ : wf Σ) (Δ : named_context) (wfΔ : wf_named Σ Δ) (Γ : context) (wfΓ : wf_local Σ Δ Γ) p prim_ty cdecl,
+        PΔ Σ Δ wfΔ ->
+        PΓ Σ Δ wfΔ Γ wfΓ ->
         primitive_constant Σ primString = Some prim_ty ->
         declared_constant Σ prim_ty cdecl ->
         primitive_invariants primString cdecl ->
-        P Σ Γ (tString p) (tConst prim_ty [])) ->
+        P Σ Δ Γ (tString p) (tConst prim_ty [])) ->
 
-    (forall Σ (wfΣ : wf Σ) (Γ : context) (wfΓ : wf_local Σ Γ) u arr def ty prim_ty cdecl,
-        PΓ Σ Γ wfΓ ->
+    (forall Σ (wfΣ : wf Σ) (Δ : named_context) (wfΔ : wf_named Σ Δ) (Γ : context) (wfΓ : wf_local Σ Δ Γ) u arr def ty prim_ty cdecl,
+        PΔ Σ Δ wfΔ ->
+        PΓ Σ Δ wfΔ Γ wfΓ ->
         primitive_constant Σ primArray = Some prim_ty ->
         declared_constant Σ prim_ty cdecl ->
         primitive_invariants primArray cdecl ->
         let s := sType (Universe.make' u) in
-        Σ ;;; Γ |- ty : tSort s ->
-        P Σ Γ ty (tSort s) ->
-        Σ ;;; Γ |- def : ty ->
-        P Σ Γ def ty ->
-        All (fun t => Σ ;;; Γ |- t : ty × P Σ Γ t ty) arr ->
-        P Σ Γ (tArray u arr def ty) (tApp (tConst prim_ty [u]) [ty])) ->
+        Σ ;;; Δ ;;; Γ |- ty : tSort s ->
+        P Σ Δ Γ ty (tSort s) ->
+        Σ ;;; Δ ;;; Γ |- def : ty ->
+        P Σ Δ Γ def ty ->
+        All (fun t => Σ ;;; Δ ;;; Γ |- t : ty × P Σ Δ Γ t ty) arr ->
+        P Σ Δ Γ (tArray u arr def ty) (tApp (tConst prim_ty [u]) [ty])) ->
 
-    (forall Σ (wfΣ : wf Σ) (Γ : context) (wfΓ : wf_local Σ Γ) (t A B : term) s,
-        PΓ Σ Γ wfΓ ->
-        Σ ;;; Γ |- t : A ->
-        P Σ Γ t A ->
-        Σ ;;; Γ |- B : tSort s ->
-        P Σ Γ B (tSort s) ->
-        Σ ;;; Γ |- A <= B ->
-        P Σ Γ t B) ->
+    (forall Σ (wfΣ : wf Σ) (Δ : named_context) (wfΔ : wf_named Σ Δ) (Γ : context) (wfΓ : wf_local Σ Δ Γ) (t A B : term) s,
+        PΔ Σ Δ wfΔ ->
+        PΓ Σ Δ wfΔ Γ wfΓ ->
+        Σ ;;; Δ ;;; Γ |- t : A ->
+        P Σ Δ Γ t A ->
+        Σ ;;; Δ ;;; Γ |- B : tSort s ->
+        P Σ Δ Γ B (tSort s) ->
+        Σ ;;; Δ ;;; Γ |- A <= B ->
+        P Σ Δ Γ t B) ->
 
-       env_prop P Pj PΓ.
+       env_prop P Pj PΔ PΓ.
 Proof.
-  intros P Pj Pdecl PΓ; unfold env_prop.
-  intros Xj XΓ.
-  intros X X0 Xcast X1 X2 X3 X4 X5 X6 X7 X8 X9 X10 X11 Xint Xfloat Xstring Xarr X12 Σ wfΣ Γ wfΓ t T H.
+  intros P Pj Pdecl PΔ PΓ. unfold env_prop.
+  intros Xj XΔ XΓ Xrel Xvar Xsort Xcast Xprod Xlam Xlet Xapp Xconst Xind Xctor Xcase Xproj Xfix Xcofix Xint Xfloat Xstring Xarr Xconv.
+  intros Σ wfΣ Δ Γ t T H.
   (* NOTE (Danil): while porting to 8.9, I had to split original "pose" into 2 pieces,
    otherwise it takes forever to execure the "pose", for some reason *)
-  pose (@Fix_F ({ Σ : global_env_ext & { wfΣ : wf Σ & { Γ & { t & { T & Σ ;;; Γ |- t : T }}}}})) as p0.
+  pose (@Fix_F ({ Σ : global_env_ext & { wfΣ : wf Σ & { Δ & { Γ & { t & { T & Σ ;;; Δ ;;; Γ |- t : T }}}}}})) as p0.
   specialize (p0 (lexprod (precompose lt (fun Σ => globenv_size (fst Σ)))
-        (fun Σ => precompose lt (fun x => typing_size x.π2.π2.π2.π2)))) as p.
-  set (foo := (Σ; wfΣ; Γ; t; _; H) : { Σ : global_env_ext & { wfΣ : wf Σ & { Γ & { t & { T & Σ ;;; Γ |- t : T }}}}}).
+        (fun Σ => precompose lt (fun x => typing_size x.π2.π2.π2.π2.π2)))) as p.
+  set (foo := (Σ; wfΣ; Δ; Γ; (t; T; H)) : { Σ : global_env_ext & { wfΣ : wf Σ & { Δ & { Γ & { t & { T & Σ ;;; Δ ;;; Γ |- t : T }}}}}}).
   change Σ with foo.π1.
-  change Γ with foo.π2.π2.π1.
-  change t with foo.π2.π2.π2.π1.
-  change T with foo.π2.π2.π2.π2.π1.
-  change H with foo.π2.π2.π2.π2.π2.
+  change Δ with foo.π2.π2.π1.
+  change Γ with foo.π2.π2.π2.π1.
+  change t with foo.π2.π2.π2.π2.π1.
+  change T with foo.π2.π2.π2.π2.π2.π1.
+  change H with foo.π2.π2.π2.π2.π2.π2.
   revert foo.
   match goal with
     |- let foo := _ in @?P foo => specialize (p (fun x => P x))
   end.
   forward p; [ | apply p; apply wf_lexprod; intros; apply wf_precompose; apply lt_wf].
-  clear p.
-  clear Σ wfΣ Γ wfΓ t T H.
-  intros (Σ & wfΣ & Γ & t & t0 & H). simpl.
+  clear p. clear Σ wfΣ Δ Γ t T H.
+  intros (Σ & wfΣ & Δ & Γ & t & t0 & H). simpl.
   intros IH. simpl in IH.
   split.
   destruct Σ as [Σ φ].
@@ -1376,12 +1479,12 @@ Proof.
   destruct wfΣ; split => //.
   rename o into ongu. rename o0 into o.
   destruct o. { constructor. }
-  rename o0 into Xg. set (wfΣ := (ongu, o) : on_global_env cumul_gen (lift_typing typing) {| universes := univs; declarations := Σ |}).
+  rename o0 into Xg. set (wfΣ := (ongu, o) : on_global_env cumul_gen (lift_typing3 typing) {| universes := univs; declarations := Σ |}).
   set (Σ':= {| universes := univs; declarations := Σ |}) in *.
   destruct Xg. rename udecl0 into udecl.
   rename on_global_decl_d0 into Xg.
   constructor; auto; try constructor; auto.
-  - unshelve eset (IH' := IH ((Σ', udecl); wfΣ; []; tSort sProp; _; _)).
+  - unshelve eset (IH' := IH ((Σ', udecl); wfΣ; []; ([]; tSort sProp; _; _))).
     shelve. simpl. apply type_Prop.
     forward IH'. constructor 1; cbn. lia.
     apply IH'; auto.
@@ -1389,7 +1492,7 @@ Proof.
     destruct d.
     + apply Xj; tas.
       apply lift_typing_impl with (1 := Xg); intros ?? Hs. split; tas.
-      specialize (IH ((Σ', udecl); wfΣ; _; _; _; Hs)).
+      specialize (IH ((Σ', udecl); wfΣ; _; _; (_; _; Hs))).
       forward IH; [constructor 1; simpl; subst Σ' Σg; cbn; lia|].
       apply IH.
     + red in Xg.
@@ -1403,68 +1506,91 @@ Proof.
         -- apply onArity in Xg.
            apply Xj; tas.
            apply lift_typing_impl with (1 := Xg); intros ?? Hs. split; tas.
-           apply (IH (_; _; _; Hs)).
+           apply (IH (_; _; _; _; Hs)).
         -- pose proof Xg.(onConstructors) as Xg'.
            eapply All2_impl; eauto.
            intros ? ? [cass tyeq onctyp oncargs oncind]; unshelve econstructor; eauto.
            { apply Xj; tas.
              apply lift_typing_impl with (1 := onctyp); intros ?? Hs. split; tas.
-             apply (IH (_; _; _; Hs)). }
+             apply (IH (_; _; _; _; Hs)). }
            { apply sorts_local_ctx_impl with (1 := oncargs); intros Γ' j' Hj'.
              apply Xj; tas.
              apply lift_typing_impl with (1 := Hj'); intros ?? Hs. split; tas.
-             apply (IH (_; _; _; Hs)). }
+             apply (IH (_; _; _; _; Hs)). }
            { eapply ctx_inst_impl with (1 := oncind); intros ?? Hj.
              apply Xj; tas.
              apply lift_typing_impl with (1 := Hj); intros ?? Hs. split; tas.
-             apply (IH (_; _; _; Hs)). }
+             apply (IH (_; _; _; _; Hs)). }
         -- pose proof (onProjections Xg); auto.
         -- pose proof (ind_sorts Xg) as Xg'. unfold check_ind_sorts in *.
            destruct Sort.to_family; auto.
            split. apply Xg'. destruct indices_matter; auto.
            eapply type_local_ctx_impl. eapply Xg'. auto. intros ?? Hj. apply Xj; tas.
            apply lift_typing_impl with (1 := Hj); intros ?? Hs. split; tas.
-           apply (IH (_; _; _; Hs)).
+           apply (IH (_; _; _; _; Hs)).
         -- apply (onIndices Xg).
       * apply All_local_env_impl with (1 := onP); intros ?? Hj. apply Xj; tas.
         apply lift_typing_impl with (1 := Hj); intros ?? Hs. split; tas.
-        apply (IH ((Σ', udecl); (wfΣ; _; _; _; Hs))).
+        apply (IH ((Σ', udecl); (wfΣ; _; _; _; _; Hs))).
         constructor 1. simpl. subst Σ' Σg; cbn; lia.
 
-  - assert (forall Γ t T (Hty : Σ ;;; Γ |- t : T),
+  - assert (forall Δ Γ t T (Hty : Σ ;;; Δ ;;; Γ |- t : T),
                typing_size Hty < typing_size H ->
-               on_global_env cumul_gen Pj Σ.1 * P Σ Γ t T).
+               on_global_env cumul_gen Pj Σ.1 * P Σ Δ Γ t T) as X1.
     { intros.
-      specialize (IH (Σ; wfΣ; _; _; _; Hty)).
+      specialize (IH (Σ; wfΣ; _; _; (_; _; Hty))).
       simpl in IH.
       forward IH.
       constructor 2. simpl. apply H0.
       intuition. }
 
-    rename X13 into X14.
-
-    assert (Xj' : forall Γ j (Hj : lift_typing typing Σ Γ j),
-        lift_typing_size (fun t T H => @typing_size cf Σ Γ t T H) _ Hj < typing_size H ->
-        Pj Σ Γ j).
-    { intros ?? Hj Hlt.
+    assert (Xj' : forall Δ Γ j (Hj : lift_typing3 typing Σ Δ Γ j),
+        lift_typing_size (fun t T H => @typing_size cf Σ Δ Γ t T H) _ Hj < typing_size H ->
+        Pj Σ Δ Γ j).
+    { intros ??? Hj Hlt.
       apply Xj; tas.
-      eapply lift_typing_size_impl with (Psize := fun t T H => @typing_size _ _ _ t T H) (tu := Hj).
+      eapply lift_typing_size_impl with (Psize := fun t T H => @typing_size _ _ _ _ t T H) (tu := Hj).
       intros ?? Hty Hlt'; split; tas.
-      apply X14 with (Hty := Hty). set (size_mid := lift_typing_size _ _ Hj) in *. lia. }
+      apply X1 with (Hty := Hty). set (size_mid := lift_typing_size _ _ Hj) in *. lia. }
     clear Xj; rename Xj' into Xj.
 
-    assert (forall Γ' t T (Hty : Σ ;;; Γ' |- t : T),
+    assert (forall Γ' t T (Hty : Σ ;;; Δ ;;; Γ' |- t : T),
       typing_size Hty <= typing_size H ->
-      PΓ Σ Γ' (typing_wf_local Hty)).
-    { intros.
+      PΔ Σ Δ (typing_wf_named Hty)) as X3.
+    { intros. apply XΔ ; tea. admit. admit. }
+    
+    assert (forall Γ' t T (Hty : Σ ;;; Δ ;;; Γ' |- t : T),
+      typing_size Hty <= typing_size H ->
+      PΓ Σ Δ (typing_wf_named Hty) Γ' (typing_wf_local Hty)) as X2.
+    { (*intros.
+      clear - wfΣ X1 Xj XΓ.
+      apply XΓ ; tas.
+      - (*pose proof (typing_wf_named_size Hty) as H1.*)
+        set (w := typing_wf_named Hty) in *. clearbody w.
+        induction w ; [constructor|constructor|constructor].
+        + apply IHw with Hty.   *) 
+      
+     admit. 
+    }
+    (*{ intros.
       pose proof (typing_wf_local_size Hty) as Hlt0.
+      pose proof (typing_wf_named_size Hty) as Hlt1.
       set (foo := typing_wf_local Hty) in *.
-      clearbody foo. assert (All_local_env_size (@typing_size cf Σ) Γ' foo < typing_size H) as Hlt by lia.
-      clear -wfΣ X14 Xj Hlt XΓ.
-      apply XΓ; tas.
-    + revert foo Hlt.
-      induction foo; simpl in *; cbn in *; constructor.
-      - simpl in *. apply IHfoo. lia.
+      set (bar := typing_wf_named Hty) in *.
+      assert (foo = typing_wf_local Hty) as Hfoo by auto.
+      assert (bar = typing_wf_named Hty) as Hbar by auto. 
+      assert (All_local_env_size (@typing_size cf Σ Δ) Γ' foo < typing_size H) as Hlt_foo by lia.
+      assert (All_named_env_size (@typing_size cf Σ) Δ bar < typing_size H) as Hlt_bar by lia.
+      clear - wfΣ X14 Xj Hbar Hfoo Hlt_bar Hlt_foo XΓ.
+      apply XΓ; tas.  
+    + admit.
+    + admit. 
+    (*+ revert bar Hlt_bar Hlt1 Eqn_bar.
+      induction bar; simpl in *; cbn in *; constructor.
+      - simpl in *. apply wf_named_inv in H. apply IHbar with (H) (Hty). ; tea.
+        4: apply typing_wf_local_size.
+        3: unfold bar. eapply (@typing_wf_named_size cf Σ Δ.
+        * lia.
       - red. apply (X14 _ _ _ t2.2.π2.1). cbn. lia.
       - simpl in *. apply IHfoo. lia.
       - red. apply (X14 _ _ _ t2.1). cbn. lia.
@@ -1473,11 +1599,27 @@ Proof.
       induction foo; cbn in *; constructor.
       1,3: apply IHfoo; lia.
       all: eapply Xj with (Hj := t2); simpl; cbn.
-      all: lia. }
+      all: lia.*)
+    + revert foo Hfoo Hlt_foo.
+      induction foo; simpl in *; cbn in *; constructor.
+      - simpl in *. eapply IHfoo ; eauto. 3: lia. admit. admit.
+      - red. apply (X14 _ _ _ _ t3.2.π2.1). cbn. lia.
+      - simpl in *. eapply IHfoo ; eauto. 3: lia. admit. admit.
+      - red. apply (X14 _ _ _ _ t3.1). cbn. lia.
+      - red. apply (X14 _ _ _ _ t3.2.π2.1). cbn. lia.
+    + revert foo Hfoo Hlt_foo.
+      induction foo; cbn in *; constructor.
+      - eapply IHfoo ; eauto. 3: lia. admit. admit.
+      - admit. 
+      - admit.
+      - admit. 
+      (*1,3: eapply IHfoo; eauto ; lia.
+      all: eapply Xj with (Hj := t2); simpl; cbn.
+      all: lia.*) }*)
 
     clear IH.
-    assert (pΓ : PΓ Σ Γ (typing_wf_local H)).
-    { apply (X13 _ _ _ H). lia. }
+    assert (pΓ : PΓ Σ Δ (typing_wf_named H) Γ (typing_wf_local H)).
+    { apply (X2 _ _ _ H). lia. }
     split; auto.
     set (wfΓ := typing_wf_local H); clearbody wfΓ.
 
@@ -1485,144 +1627,173 @@ Proof.
       try solve [  match reverse goal with
                     H : _ |- _ => eapply H
                   end; eauto;
-                  unshelve eapply X14; simpl; auto with arith].
+                  unshelve eapply X2; simpl; auto with arith].
 
     all: try solve [ match reverse goal with H : _ |- _ => eapply H end;
-      eauto; [ unshelve eapply Xj | unshelve eapply X14 ]; simpl; auto with arith ].
+      eauto; [ unshelve eapply Xj | unshelve eapply X2 ]; simpl; auto with arith ].
 
-    -- clear X X0 Xcast X1 X2 X3 X5 X6 X7 X8 X9 X10 X11 X12 X13 Xj.
-       eapply X4 with t_ty t0; eauto. clear X4.
-       unshelve eapply X14; simpl; auto with arith.
-       simpl in X14.
-       assert(X: forall Γ0, wf_local Σ Γ0 ->
-              forall t1 T (Hty : Σ;;; Γ0 |- t1 : T),
-                typing_size Hty < S ((typing_spine_size (@typing_size cf) Σ Γ t_ty l t' t0)) ->
-                on_global_env cumul_gen Pj Σ.1 * P Σ Γ0 t1 T). {
-       intros. unshelve eapply X14; eauto. lia. }
-       clear X14. simpl in pΓ. clear n e H pΓ.
-       induction t0; constructor.
-       unshelve eapply X; clear X; simpl; auto with arith.
-       unshelve eapply X; clear X; simpl; auto with arith.
-       eapply IHt0; eauto. intros. eapply (X _ X0 _ _ Hty) ; eauto. simpl. lia.
+    --clear p0 Xrel Xvar Xsort Xprod Xlam Xlet Xapp Xconst Xind Xctor Xcase Xproj Xfix Xcofix Xint Xfloat Xstring Xarr Xconv.
+      unshelve eapply Xcast ; eauto.
+      * apply (typing_wf_named H).  
+      * unshelve eapply X1 ; simpl ; eauto with arith.
+      * unshelve eapply X1 ; simpl ; eauto with arith.
 
-    -- eapply X5; eauto.
-       specialize (X14 [] _ _ (type_Prop _)).
-       simpl in X14. forward X14; auto. unfold All_local_env_size at 1, All_local_env_size_gen. lia. apply X14.
+    --clear p0 Xrel Xvar Xsort Xcast Xlam Xlet Xapp Xconst Xind Xctor Xcase Xproj Xfix Xcofix Xint Xfloat Xstring Xarr Xconv.
+      eapply Xprod ; eauto.
+      unshelve eapply Xj; simpl; auto with arith.
+      simpl in X1. unshelve eapply X1 ; eauto with arith.
+      
+    --clear p0 Xrel Xvar Xsort Xcast Xprod Xlet Xapp Xconst Xind Xctor Xcase Xproj Xfix Xcofix Xint Xfloat Xstring Xarr Xconv.
+      eapply Xlam ; eauto.
+      unshelve eapply Xj ; simpl ; eauto with arith.
+      simpl in X1. unshelve eapply X1 ; eauto with arith.
+    
+    --clear p0 Xrel Xvar Xsort Xcast Xprod Xlam Xapp Xconst Xind Xctor Xcase Xproj Xfix Xcofix Xint Xfloat Xstring Xarr Xconv.
+      eapply Xlet ; eauto.
+      unshelve eapply Xj ; simpl ; eauto with arith.
+      simpl in X1. unshelve eapply X1 ; eauto with arith.
+  
+    --clear p0 Xrel Xvar Xsort Xcast Xprod Xlam Xlet Xconst Xind Xctor Xcase Xproj Xfix Xcofix Xint Xfloat Xstring Xarr Xconv.
+      unshelve eapply (Xapp Σ wfΣ Δ _ Γ _ t l t_ty t' _ _ _ _ t0) ; eauto ; clear Xapp.
+      eapply typing_wf_named ; tea.
+      simpl in X1. eapply X1 ; eauto with arith.
+      admit.
+      (*simpl in X1 ; simpl in X2 ; clear Xj n. 
+      generalize dependent t.
+      induction t0.
+      ++(*simpl in X1. unshelve eapply X1 ; eauto with arith.*) admit.
+      ++(*simpl in X1. unshelve eapply X1 ; eauto with arith.*) admit.
+      ++(*unshelve eapply (IHt0 wfΓ (mkApps t2 [hd])) ; eauto.
+        About type_App.  
+        Print typing_spine.*)*)
 
-    -- eapply X6; eauto.
-       specialize (X14 [] _ _ (type_Prop _)).
-       simpl in X14. forward X14; auto. unfold All_local_env_size at 1, All_local_env_size_gen. lia. apply X14.
+    --clear p0 Xrel Xvar Xsort Xcast Xprod Xlam Xlet Xapp Xind Xctor Xcase Xproj Xfix Xcofix Xint Xfloat Xstring Xarr Xconv.
+      unshelve eapply (Xconst Σ wfΣ Δ (typing_wf_named _) Γ a0) ; eauto. 
+      specialize (X1 [] [] _ _ (type_Prop Σ)). apply X1.
+      rewrite typing_size_Prop. simpl ; lia.
+      
+    --clear p0 Xrel Xvar Xsort Xcast Xprod Xlam Xlet Xapp Xconst Xctor Xcase Xproj Xfix Xcofix Xint Xfloat Xstring Xarr Xconv.
+      unshelve eapply (Xind Σ wfΣ Δ (typing_wf_named _) Γ a0) ; eauto. 
+      specialize (X1 [] [] _ _ (type_Prop Σ)). apply X1.
+      rewrite typing_size_Prop. simpl; lia.
+      
+    --clear p0 Xrel Xvar Xsort Xcast Xprod Xlam Xlet Xapp Xconst Xind Xcase Xproj Xfix Xcofix Xint Xfloat Xstring Xarr Xconv.
+      unshelve eapply (Xctor Σ wfΣ Δ (typing_wf_named _) Γ a0) ; eauto. 
+      specialize (X1 [] [] _ _ (type_Prop Σ)). apply X1.
+      rewrite typing_size_Prop. simpl; lia.
+    
+    --clear p0 Xrel Xvar Xsort Xcast Xprod Xlam Xlet Xapp Xconst Xind Xctor Xproj Xfix Xcofix Xint Xfloat Xstring Xarr Xconv.
+      simpl in pΓ.
+      eapply (Xcase Σ wfΣ Δ (typing_wf_named _) Γ (typing_wf_local _) ci); eauto.
+      ++specialize (X1 [] [] _ _ (type_Prop Σ)). apply X1.
+        rewrite typing_size_Prop. simpl. rewrite <- Nat.succ_lt_mono.
+        rewrite Nat.max_lt_iff ; left. apply typing_size_pos.
+      ++assert (forall Γ' t T (Hty : Σ ;;; Δ ;;; Γ' |- t : T),
+           typing_size Hty <= ctx_inst_size typing (@typing_size _) c1 ->
+           P Σ Δ Γ' t T).
+        { intros. eapply (X1 _ _ _ _ Hty). simpl.
+          change (fun _ _ _ _ _ H => typing_size H) with (@typing_size cf).
+          lia. }
+        clear -X c1.
+        revert c1 X.
+        generalize (List.rev (subst_instance (puinst p) (ind_params mdecl ,,, ind_indices idecl : context))).
+        generalize (pparams p ++ indices).
+        intros l c ctxi IH; induction ctxi; constructor; eauto.
+        * split; tas. eapply (IH _ _ _ t0); simpl; auto. lia.
+        * eapply IHctxi. intros. eapply (IH _ _ _ Hty). simpl. lia.
+        * eapply IHctxi. intros. eapply (IH _ _ _ Hty). simpl. lia.
+        ++ simpl in X1. simpl in pΓ. auto. eapply (X1 _ _ _ _ H); eauto. simpl; auto with arith.
+      ++ eapply (X2 _ _ _ H); eauto. simpl. subst predctx. lia.
+      ++ eapply (X1 _ _ _ _ H0); simpl. lia.
+      ++ clear X3 X2 Xj. revert a X1. clear. intros.
+         subst ptm predctx.
+         Opaque case_branch_type.
+         simpl in X1.
+         Transparent case_branch_type.
+         induction a0; simpl in *.
+         ** constructor.
+         ** destruct r0 as [[? ?] ?]. constructor.
+             --- intuition eauto.
+                 +++ eapply (X1 _ _ _ _ t); eauto. clear -X1. simpl; auto with arith.
+                     lia.
+                 +++ eapply (X1 _ _ _ _ t0); eauto. simpl; auto with arith.
+                     lia.
+             --- apply IHa0. auto. intros.
+                 eapply (X1 _ _ _ _ Hty). lia.
 
-    -- eapply X7; eauto.
-       specialize (X14 [] _ _ (type_Prop _)).
-       simpl in X14. forward X14; auto. unfold All_local_env_size at 1, All_local_env_size_gen. lia. apply X14.
-
-    -- simpl in pΓ.
-       eapply (X8 Σ wfΣ Γ (typing_wf_local H0) ci); eauto.
-       ++ eapply (X14 _ _ _ H0); eauto. simpl; auto with arith. lia.
-       ++ clear -c1 X14.
-        assert (forall Γ' t T (Hty : Σ;;; Γ' |- t : T),
-           typing_size Hty <= ctx_inst_size _ (@typing_size _) c1 ->
-         P Σ Γ' t T).
-       { intros. eapply (X14 _ _ _ Hty). simpl.
-         change (fun _ _ _ _ H => typing_size H) with (@typing_size cf).
-         lia. }
-       clear -X c1.
-       revert c1 X.
-       generalize (List.rev (subst_instance (puinst p) (ind_params mdecl ,,, ind_indices idecl : context))).
-       generalize (pparams p ++ indices).
-       intros l c ctxi IH; induction ctxi; constructor; eauto.
-       * split; tas. eapply (IH _ _ _ t0); simpl; auto. lia.
-       * eapply IHctxi. intros. eapply (IH _ _ _ Hty). simpl. lia.
-       * eapply IHctxi. intros. eapply (IH _ _ _ Hty). simpl. lia.
-
-       ++ simpl in X13. simpl in pΓ. auto. eapply (X14 _ _ _ H); eauto. simpl; auto with arith.
-       ++ simpl in *.
-         eapply (X13 _ _ _ H); eauto. simpl. subst predctx. lia.
-       ++ eapply (X14 _ _ _ H0); simpl. lia.
-       ++ clear X13 Xj. revert a X14. clear. intros.
-          subst ptm predctx.
-          Opaque case_branch_type.
-          simpl in X14.
-          Transparent case_branch_type.
-          induction a0; simpl in *.
-          ** constructor.
-          ** destruct r0 as [[? ?] ?]. constructor.
-              --- intuition eauto.
-                  +++ eapply (X14 _ _ _ t); eauto. clear -X14. simpl; auto with arith.
-                      lia.
-                  +++ eapply (X14 _ _ _ t0); eauto. simpl; auto with arith.
-                      lia.
-              --- apply IHa0. auto. intros.
-                  eapply (X14 _ _ _ Hty). lia.
-
-    -- eapply X9; eauto.
-       specialize (X14 [] _ _ (type_Prop _)).
-       simpl in X14. forward X14; auto. pose (typing_size_pos H). unfold All_local_env_size at 1, All_local_env_size_gen. lia. apply X14.
-       unshelve eapply X14; eauto.
-
-    -- clear X X0 Xcast X1 X2 X3 X4 X5 X6 X7 X8 X9 X11 X12.
-       eapply X10; eauto; clear X10.
-      * assert (forall j Hj, lift_typing_size (fun t T H => @typing_size cf Σ Γ t T H) j Hj <
-                  S (all_size _ (fun x p => on_def_type_size (@typing_size _ Σ) _ _ p) a0) ->
-                  Pj Σ Γ j).
-        { intros. eapply Xj with (Hj := Hj); eauto. simpl. lia. }
-        clear -a0 X.
-        induction a0; constructor.
-        ++ eapply X with (Hj := p). cbn.
-          unfold on_def_type_sorting_size, lift_sorting_size, option_default_size in *.
-          cbn in *. lia.
-        ++ apply IHa0. intros. eapply X with (Hj := Hj); eauto.
-          simpl. lia.
-      * simpl in X14.
-        assert (forall Γ, wf_local Σ Γ ->
-                forall j Hj, lift_typing_size (fun t T H => @typing_size cf Σ Γ t T H) j Hj <
-                S (all_size (on_def_body (lift_typing typing _) _ _) (fun x p => on_def_body_size (@typing_size cf Σ) _ _ _ p) a1) ->
-                Pj Σ Γ j).
-        { intros. eapply Xj with (Hj := Hj); eauto. simpl. lia. }
-        clear -a1 X.
-        remember (fix_context mfix) as mfixcontext eqn:e. clear e.
-        induction a1; constructor.
-        ++ eapply X with (Hj := p). 1: eapply typing_wf_local, p.1. cbn. lia.
-        ++ apply IHa1. intros. eapply X with (Hj := Hj); eauto.
-          simpl. lia.
-
-      -- clear X X0 Xcast X1 X2 X3 X4 X5 X6 X7 X8 X9 X10 X12.
-         eapply X11; eauto; clear X11. simpl in *.
-      * assert (forall j Hj, lift_typing_size (fun t T H => @typing_size cf Σ Γ t T H) j Hj <
-                  S (all_size _ (fun x p => on_def_type_size (@typing_size _ Σ) _ _ p) a0) ->
-                  Pj Σ Γ j).
-        { intros. eapply Xj with (Hj := Hj); eauto. simpl. lia. }
-        clear -a0 X.
-        induction a0; constructor.
-        ++ eapply X with (Hj := p). cbn.
-          unfold on_def_type_sorting_size, lift_sorting_size, option_default_size in *.
-          cbn in *. lia.
-        ++ apply IHa0. intros. eapply X with (Hj := Hj); eauto.
-          simpl. lia.
-      * simpl in X14.
-        assert (forall Γ, wf_local Σ Γ ->
-                forall j Hj, lift_typing_size (fun t T H => @typing_size cf Σ Γ t T H) j Hj <
-                S (all_size (on_def_body (lift_typing typing _) _ _) (fun x p => on_def_body_size (@typing_size cf _) _ _ _ p) a1) ->
-                Pj Σ Γ j).
+    --clear p0 Xrel Xvar Xsort Xcast Xprod Xlam Xlet Xapp Xconst Xind Xctor Xcase Xfix Xcofix Xint Xfloat Xstring Xarr Xconv.
+      eapply Xproj; eauto; clear Xproj.
+      ++specialize (X1 [] [] _ _ (type_Prop _)). apply X1. 
+        rewrite typing_size_Prop. simpl. generalize (typing_size_pos H). lia.
+      ++simpl in X1. admit.
+      
+    --clear p0 Xrel Xvar Xsort Xcast Xprod Xlam Xlet Xapp Xconst Xind Xctor Xcase Xproj Xcofix Xint Xfloat Xstring Xarr Xconv.
+      eapply Xfix; eauto; clear Xfix.
+      ++assert (forall j Hj, lift_typing_size (fun t T H => @typing_size cf Σ Δ Γ t T H) j Hj <
+                  S (all_size _ (fun x p => on_def_type_size (@typing_size _ Σ Δ) _ _ p) a1) ->
+                  Pj Σ Δ Γ j).
         { intros. eapply Xj with (Hj := Hj); eauto. simpl. lia. }
         clear -a1 X.
-        remember (fix_context mfix) as mfixcontext eqn:e. clear e.
         induction a1; constructor.
-        ++ eapply X with (Hj := p). 1: eapply typing_wf_local, p.1. cbn. lia.
-        ++ apply IHa1. intros. eapply X with (Hj := Hj); eauto.
+        **eapply X with (Hj := p). cbn.
+           unfold on_def_type_sorting_size, lift_sorting_size, option_default_size in *.
+           cbn in *. lia.
+        **apply IHa1. intros. eapply X with (Hj := Hj); eauto.
+           simpl. lia.
+      ++assert (forall Γ, wf_local Σ Δ Γ ->
+                forall j Hj, lift_typing_size (fun t T H => @typing_size cf Σ Δ Γ t T H) j Hj <
+                S (all_size (on_def_body (lift_typing3 typing Σ Δ) _ _) (fun x p => on_def_body_size (@typing_size cf Σ Δ) _ _ _ p) a2) ->
+                Pj Σ Δ Γ j).
+        { intros. eapply Xj with (Hj := Hj); eauto. simpl. lia. }
+        clear -a2 X.
+        remember (fix_context mfix) as mfixcontext eqn:e. clear e.
+        induction a2; constructor.
+        **eapply X with (Hj := p). 1: eapply typing_wf_local, p.1. cbn. lia.
+        **apply IHa2. intros. eapply X with (Hj := Hj); eauto.
           simpl. lia.
-      -- eapply Xarr; tea.
-        * eapply (X14 _ _ _ H). simpl. subst s; lia.
-        * eapply (X14 _ _ _ H0). simpl. subst s; lia.
-        * assert (Xi : forall t (Hty : Σ;;; Γ |- t : ty), typing_size Hty < S (all_size _ (fun t p => typing_size p) a0) ->
-                  P Σ Γ t ty).
-          { intros ? Hty ?; eapply (X14 _ _ _ Hty). simpl. lia. }
-          clear -Xi a0.
-          induction a0; constructor; eauto.
-          + split => //. eapply (Xi _ p). cbn. lia.
-          + eapply IHa0. intros. eapply (Xi _ Hty). simpl. lia.
-Qed.
+
+    --clear p0 Xrel Xvar Xsort Xcast Xprod Xlam Xlet Xapp Xconst Xind Xctor Xcase Xproj Xfix Xint Xfloat Xstring Xarr Xconv.
+      eapply Xcofix; eauto; clear Xcofix. simpl in *.
+      ++assert (forall j Hj, lift_typing_size (fun t T H => @typing_size cf Σ Δ Γ t T H) j Hj <
+                  S (all_size _ (fun x p => on_def_type_size (@typing_size _ Σ Δ) _ _ p) a1) ->
+                  Pj Σ Δ Γ j).
+        { intros. eapply Xj with (Hj := Hj); eauto. simpl. lia. }
+        clear -a1 X.
+        induction a1; constructor.
+        **eapply X with (Hj := p). cbn.
+          unfold on_def_type_sorting_size, lift_sorting_size, option_default_size in *.
+          cbn in *. lia.
+        **apply IHa1. intros. eapply X with (Hj := Hj); eauto.
+          simpl. lia.
+      ++assert (forall Γ, wf_local Σ Δ Γ ->
+                forall j Hj, lift_typing_size (fun t T H => @typing_size cf Σ Δ Γ t T H) j Hj <
+                S (all_size (on_def_body (lift_typing3 typing Σ Δ) _ _) (fun x p => on_def_body_size (@typing_size cf Σ Δ) _ _ _ p) a2) ->
+                Pj Σ Δ Γ j).
+        { intros. eapply Xj with (Hj := Hj); eauto. simpl. lia. }
+        clear -a2 X.
+        remember (fix_context mfix) as mfixcontext eqn:e. clear e.
+        induction a2; constructor.
+        **eapply X with (Hj := p). 1: eapply typing_wf_local, p.1. cbn. lia.
+        **apply IHa2. intros. eapply X with (Hj := Hj); eauto.
+          simpl. lia.
+
+    --clear p0 Xrel Xvar Xsort Xcast Xprod Xlam Xlet Xapp Xconst Xind Xctor Xcase Xproj Xfix Xcofix Xint Xstring Xfloat Xconv.
+      eapply (Xarr Σ wfΣ Δ (typing_wf_named _) Γ); eauto ; clear Xarr.
+      * eapply (X1 _ _ _ _ H). simpl. subst s; lia.
+      * eapply (X1 _ _ _ _ H0). simpl. subst s; lia.
+      * assert (Xi : forall t (Hty : Σ ;;; Δ ;;; Γ |- t : ty), typing_size Hty < S (all_size _ (fun t p => typing_size p) a1) ->
+                  P Σ Δ Γ t ty).
+        { intros ? Hty ?; eapply (X1 _ _ _ _ Hty). simpl. lia. }
+        clear -Xi a1.
+        induction a1; constructor; eauto.
+        + split => //. eapply (Xi _ p). cbn. lia.
+        + unshelve eapply IHa1. intros. eapply (Xi _ Hty). simpl. lia.
+    
+    --clear p0 Xrel Xvar Xsort Xcast Xprod Xlam Xlet Xapp Xconst Xind Xctor Xcase Xproj Xfix Xcofix Xint Xstring Xfloat Xarr.
+      eapply Xconv ; eauto ; clear Xconv.
+      ++unshelve eapply (X1 _ _ _ _ H). simpl. lia.
+      ++unshelve eapply (X1 _ _ _ _ H0). simpl. lia.
+Admitted.
 
 Arguments on_global_env {cf} Pcmp P !g.
 
